@prefix cc: <http://creativecommons.org/ns#> .
@prefix iss-sdcr: <http://data.europa.eu/949/iss/concepts/safety-direct-cause-reported-types/> .
@prefix dct: <http://purl.org/dc/terms/> .
@prefix rdf: <http://www.w3.org/1999/02/22-rdf-syntax-ns#> .
@prefix owl: <http://www.w3.org/2002/07/owl#> .
@prefix xsd: <http://www.w3.org/2001/XMLSchema#> .
@prefix skos: <http://www.w3.org/2004/02/skos/core#> .
@prefix rdfs: <http://www.w3.org/2000/01/rdf-schema#> .

iss-sdcr:DirectCauseReportedTypes
    cc:license <https://creativecommons.org/licenses/by/4.0/> ;
    dct:issued "2024-04-04"^^xsd:date ;
    dct:modified "2025-04-22"^^xsd:date ;
    dct:modified "2024-09-03"^^xsd:date ;
    dct:modified "2024-08-29"^^xsd:date ;
    dct:title "Concept scheme grouping safety direct cause of types"@en ;
    rdf:type skos:ConceptScheme ;
    rdfs:comment "Controlled SKOS-based vocabulary defined by the European Union Agency for Railways to describe concepts related to the Information Sharing System (ISS) in accordance with the draft delegated act of the future CSM ASLP Regulation."@en ;
    rdfs:label "Safety direct cause event Types"@en ;
    skos:hasTopConcept iss-sdcr:B ;
    skos:prefLabel "Safety direct cause of event Types"@en .

<http://data.europa.eu/949/iss/concepts/safety-direct-cause-reported-types/B>
    rdf:type skos:Concept ;
    skos:inScheme iss-sdcr:DirectCauseReportedTypes ;
    skos:prefLabel "Direct cause reported types"@en ;
    skos:topConceptOf iss-sdcr:DirectCauseReportedTypes .

<http://data.europa.eu/949/iss/concepts/safety-direct-cause-reported-types/B.1>
    rdf:type skos:Concept ;
    skos:broader <http://data.europa.eu/949/iss/concepts/safety-direct-cause-reported-types/B> ;
    skos:definition "An operation failure event falling within the B.1 sub-categories for which detailed information is not (yet) available."@en ;
    skos:inScheme iss-sdcr:DirectCauseReportedTypes ;
    skos:notation "B.1"^^xsd:token ;
    skos:prefLabel "B.1-Operation failures"@en .

<http://data.europa.eu/949/iss/concepts/safety-direct-cause-reported-types/B.1.1>
    rdf:type skos:Concept ;
    skos:broader <http://data.europa.eu/949/iss/concepts/safety-direct-cause-reported-types/B.1> ;
    skos:definition "A failure to operate the infrastructure falling within the B.1.1 sub-categories for which detailed information is not (yet) available."@en ;
    skos:inScheme iss-sdcr:DirectCauseReportedTypes ;
    skos:notation "B.1.1"^^xsd:token ;
    skos:prefLabel "B.1.1-Failure to operate the infrastructure"@en .

<http://data.europa.eu/949/iss/concepts/safety-direct-cause-reported-types/B.1.1.1>
    rdf:type skos:Concept ;
    skos:broader <http://data.europa.eu/949/iss/concepts/safety-direct-cause-reported-types/B.1.1> ;
    skos:definition "Any occasion when a train/vehicle is directed on a route that was not planned."@en ;
    skos:inScheme iss-sdcr:DirectCauseReportedTypes ;
    skos:notation "B.1.1.1"^^xsd:token ;
    skos:prefLabel "B.1.1.1-Improper routing"@en .

<http://data.europa.eu/949/iss/concepts/safety-direct-cause-reported-types/B.1.1.2>
    rdf:type skos:Concept ;
    skos:broader <http://data.europa.eu/949/iss/concepts/safety-direct-cause-reported-types/B.1.1> ;
    skos:definition "On track machine(s) or other object(s) used during infrastructure activities positioned outside the authorised area"@en ;
    skos:inScheme iss-sdcr:DirectCauseReportedTypes ;
    skos:notation "B.1.1.2"^^xsd:token ;
    skos:prefLabel "B.1.1.2-On track plant incorrectly outside possession"@en .

<http://data.europa.eu/949/iss/concepts/safety-direct-cause-reported-types/B.1.1.3>
    rdf:type skos:Concept ;
    skos:broader <http://data.europa.eu/949/iss/concepts/safety-direct-cause-reported-types/B.1.1> ;
    skos:definition "Any occasion when a switch in a wrong position is run over in trailing direction (converging points) unintentionally."@en ;
    skos:inScheme iss-sdcr:DirectCauseReportedTypes ;
    skos:notation "B.1.1.3"^^xsd:token ;
    skos:prefLabel "B.1.1.3-Pushed switch"@en .

<http://data.europa.eu/949/iss/concepts/safety-direct-cause-reported-types/B.1.1.4>
    rdf:type skos:Concept ;
    skos:broader <http://data.europa.eu/949/iss/concepts/safety-direct-cause-reported-types/B.1.1> ;
    skos:definition "Any occasion when a passenger train is stopped in a tunnel for more than 10 minutes. Stops in underground stations should be excluded."@en ;
    skos:inScheme iss-sdcr:DirectCauseReportedTypes ;
    skos:notation "B.1.1.4"^^xsd:token ;
    skos:prefLabel "B.1.1.4-Long stop in tunnel"@en .

<http://data.europa.eu/949/iss/concepts/safety-direct-cause-reported-types/B.1.2>
    rdf:type skos:Concept ;
    skos:broader <http://data.europa.eu/949/iss/concepts/safety-direct-cause-reported-types/B.1> ;
    skos:definition "A failure to operate a train or rail vehicle falling within the B.1.2 sub-categories for which detailed information is not (yet) available."@en ;
    skos:inScheme iss-sdcr:DirectCauseReportedTypes ;
    skos:notation "B.1.2"^^xsd:token ;
    skos:prefLabel "B.1.2-Failure to operate a train or rail vehicle(s)"@en .

<http://data.europa.eu/949/iss/concepts/safety-direct-cause-reported-types/B.1.2.1>
    rdf:type skos:Concept ;
    skos:broader <http://data.europa.eu/949/iss/concepts/safety-direct-cause-reported-types/B.1.2> ;
    skos:definition "Any occasion when any part of a train or rail vehicle proceeds beyond its authorised movement and travels beyond the danger point."@en ;
    skos:inScheme iss-sdcr:DirectCauseReportedTypes ;
    skos:notation "B.1.2.1"^^xsd:token ;
    skos:prefLabel "B.1.2.1-Signal passed at danger with passing of a danger point"@en .

<http://data.europa.eu/949/iss/concepts/safety-direct-cause-reported-types/B.1.2.10>
    rdf:type skos:Concept ;
    skos:broader <http://data.europa.eu/949/iss/concepts/safety-direct-cause-reported-types/B.1.2> ;
    skos:definition "Any occasion when a passenger train is stopped in a tunnel for more than 10 minutes. Stops in underground stations should be excluded."@en ;
    skos:inScheme iss-sdcr:DirectCauseReportedTypes ;
    skos:notation "B.1.2.10"^^xsd:token ;
    skos:prefLabel "B.1.2.10-Long stop in tunnel"@en .

<http://data.europa.eu/949/iss/concepts/safety-direct-cause-reported-types/B.1.2.11>
    rdf:type skos:Concept ;
    skos:broader <http://data.europa.eu/949/iss/concepts/safety-direct-cause-reported-types/B.1.2> ;
    skos:definition "Any situation in which a brake application by the driver is exceeding applicable limits"@en ;
    skos:inScheme iss-sdcr:DirectCauseReportedTypes ;
    skos:notation "B.1.2.11"^^xsd:token ;
    skos:prefLabel "B.1.2.11-Severe brake"@en .

<http://data.europa.eu/949/iss/concepts/safety-direct-cause-reported-types/B.1.2.12>
    rdf:type skos:Concept ;
    skos:broader <http://data.europa.eu/949/iss/concepts/safety-direct-cause-reported-types/B.1.2> ;
    skos:definition "Any situation in which the brake system is not set correctly in relation with the load"@en ;
    skos:inScheme iss-sdcr:DirectCauseReportedTypes ;
    skos:notation "B.1.2.12"^^xsd:token ;
    skos:prefLabel "B.1.2.12-Brake not correctly set for load"@en .

<http://data.europa.eu/949/iss/concepts/safety-direct-cause-reported-types/B.1.2.2>
    rdf:type skos:Concept ;
    skos:broader <http://data.europa.eu/949/iss/concepts/safety-direct-cause-reported-types/B.1.2> ;
    skos:definition "Any occasion when any part of a train or rail vehicle proceeds beyond its authorised movement but does not travel beyond the danger point"@en ;
    skos:inScheme iss-sdcr:DirectCauseReportedTypes ;
    skos:notation "B.1.2.2"^^xsd:token ;
    skos:prefLabel "B.1.2.2-Signal passed at danger without passing a danger point"@en .

<http://data.europa.eu/949/iss/concepts/safety-direct-cause-reported-types/B.1.2.3>
    rdf:type skos:Concept ;
    skos:broader <http://data.europa.eu/949/iss/concepts/safety-direct-cause-reported-types/B.1.2> ;
    skos:definition "Any uncontrolled movement of a train or rail vehicle over a distance of at least one meter."@en ;
    skos:inScheme iss-sdcr:DirectCauseReportedTypes ;
    skos:notation "B.1.2.3"^^xsd:token ;
    skos:prefLabel "B.1.2.3-Runaway"@en .

<http://data.europa.eu/949/iss/concepts/safety-direct-cause-reported-types/B.1.2.4>
    rdf:type skos:Concept ;
    skos:broader <http://data.europa.eu/949/iss/concepts/safety-direct-cause-reported-types/B.1.2> ;
    skos:definition "Any occasion when a train runs with a speed higher than the maximum authorized speed or design speed."@en ;
    skos:inScheme iss-sdcr:DirectCauseReportedTypes ;
    skos:notation "B.1.2.4"^^xsd:token ;
    skos:prefLabel "B.1.2.4-Over-speeding"@en .

<http://data.europa.eu/949/iss/concepts/safety-direct-cause-reported-types/B.1.2.5>
    rdf:type skos:Concept ;
    skos:broader <http://data.europa.eu/949/iss/concepts/safety-direct-cause-reported-types/B.1.2> ;
    skos:definition "Any situation in which goods are improperly loaded (not in accordance with the applicable safety requirements)"@en ;
    skos:inScheme iss-sdcr:DirectCauseReportedTypes ;
    skos:notation "B.1.2.5"^^xsd:token ;
    skos:prefLabel "B.1.2.5-Loading irregularity"@en .

<http://data.europa.eu/949/iss/concepts/safety-direct-cause-reported-types/B.1.2.6>
    rdf:type skos:Concept ;
    skos:broader <http://data.europa.eu/949/iss/concepts/safety-direct-cause-reported-types/B.1.2> ;
    skos:definition "Any situation in which a train composition does not respect the applicable safety requirements. It excludes all events already covered by other category B events (e.g. 'Brake not correctly set for load’ or ‘Failure of the braking system’)."@en ;
    skos:inScheme iss-sdcr:DirectCauseReportedTypes ;
    skos:notation "B.1.2.6"^^xsd:token ;
    skos:prefLabel "B.1.2.6-Train composition Failure"@en .

<http://data.europa.eu/949/iss/concepts/safety-direct-cause-reported-types/B.1.2.7>
    rdf:type skos:Concept ;
    skos:broader <http://data.europa.eu/949/iss/concepts/safety-direct-cause-reported-types/B.1.2> ;
    skos:definition "When this situation is taking place unintentionally or without specific RU procedure to be followed "@en ;
    skos:inScheme iss-sdcr:DirectCauseReportedTypes ;
    skos:notation "B.1.2.7"^^xsd:token ;
    skos:prefLabel "B.1.2.7-Train available for boarding or alignment outside platform "@en .

<http://data.europa.eu/949/iss/concepts/safety-direct-cause-reported-types/B.1.2.8>
    rdf:type skos:Concept ;
    skos:broader <http://data.europa.eu/949/iss/concepts/safety-direct-cause-reported-types/B.1.2> ;
    skos:definition "Any situation in which a person is entrapped in door(s) of a railway vehicle"@en ;
    skos:inScheme iss-sdcr:DirectCauseReportedTypes ;
    skos:notation "B.1.2.8"^^xsd:token ;
    skos:prefLabel "B.1.2.8-Person entrapment in door"@en .

<http://data.europa.eu/949/iss/concepts/safety-direct-cause-reported-types/B.1.2.9>
    rdf:type skos:Concept ;
    skos:broader <http://data.europa.eu/949/iss/concepts/safety-direct-cause-reported-types/B.1.2> ;
    skos:definition "Any situation in which a train departs or runs with an unsupervised open door"@en ;
    skos:inScheme iss-sdcr:DirectCauseReportedTypes ;
    skos:notation "B.1.2.9"^^xsd:token ;
    skos:prefLabel "B.1.2.9-Train running with open door"@en .

<http://data.europa.eu/949/iss/concepts/safety-direct-cause-reported-types/B.2>
    rdf:type skos:Concept ;
    skos:broader <http://data.europa.eu/949/iss/concepts/safety-direct-cause-reported-types/B> ;
    skos:definition "A technical failure of the rolling stock falling within the B.2 sub-categories for which detailed information is not (yet) available."@en ;
    skos:inScheme iss-sdcr:DirectCauseReportedTypes ;
    skos:notation "B.2"^^xsd:token ;
    skos:prefLabel "B.2-Technical Failure of the rolling stocks"@en .

<http://data.europa.eu/949/iss/concepts/safety-direct-cause-reported-types/B.2.1>
    rdf:type skos:Concept ;
    skos:broader <http://data.europa.eu/949/iss/concepts/safety-direct-cause-reported-types/B.2> ;
    skos:definition "A failure of the wheelset falling within the B.2.1 sub-categories for which detailed information is not (yet) available."@en ;
    skos:inScheme iss-sdcr:DirectCauseReportedTypes ;
    skos:notation "B.2.1"^^xsd:token ;
    skos:prefLabel "B.2.1-Failure of the wheelset"@en .

<http://data.europa.eu/949/iss/concepts/safety-direct-cause-reported-types/B.2.1.1>
    rdf:type skos:Concept ;
    skos:broader <http://data.europa.eu/949/iss/concepts/safety-direct-cause-reported-types/B.2.1> ;
    skos:definition "A crack/defect affecting the wheel and exceeding the applicable limits. Note: this category excludes broken wheels resulting from hot wheels"@en ;
    skos:inScheme iss-sdcr:DirectCauseReportedTypes ;
    skos:notation "B.2.1.1"^^xsd:token ;
    skos:prefLabel "B.2.1.1-Broken wheel on rolling stock "@en .

<http://data.europa.eu/949/iss/concepts/safety-direct-cause-reported-types/B.2.1.2>
    rdf:type skos:Concept ;
    skos:broader <http://data.europa.eu/949/iss/concepts/safety-direct-cause-reported-types/B.2.1> ;
    skos:definition "A crack/defect affecting the axle and exceeding the applicable limits Note: this category excludes broken axles resulting from hot axles boxes."@en ;
    skos:inScheme iss-sdcr:DirectCauseReportedTypes ;
    skos:notation "B.2.1.2"^^xsd:token ;
    skos:prefLabel "B.2.1.2-Broken axle on rolling stock"@en .

<http://data.europa.eu/949/iss/concepts/safety-direct-cause-reported-types/B.2.1.3>
    rdf:type skos:Concept ;
    skos:broader <http://data.europa.eu/949/iss/concepts/safety-direct-cause-reported-types/B.2.1> ;
    skos:definition "Any situation in which the axle and/or the wheel temperature goes outside the defined range for normal operations (including when it results in damage to the wheel or axle)."@en ;
    skos:inScheme iss-sdcr:DirectCauseReportedTypes ;
    skos:notation "B.2.1.3"^^xsd:token ;
    skos:prefLabel "B.2.1.3-Hot axle box and/or hot wheel"@en .

<http://data.europa.eu/949/iss/concepts/safety-direct-cause-reported-types/B.2.1.4>
    rdf:type skos:Concept ;
    skos:broader <http://data.europa.eu/949/iss/concepts/safety-direct-cause-reported-types/B.2.1> ;
    skos:definition "Any situation in which a failure of the bogie is detected. Note: this category excludes failure of the suspension system"@en ;
    skos:inScheme iss-sdcr:DirectCauseReportedTypes ;
    skos:notation "B.2.1.4"^^xsd:token ;
    skos:prefLabel "B.2.1.4-Failure of the bogie"@en .

<http://data.europa.eu/949/iss/concepts/safety-direct-cause-reported-types/B.2.1.5>
    rdf:type skos:Concept ;
    skos:broader <http://data.europa.eu/949/iss/concepts/safety-direct-cause-reported-types/B.2.1> ;
    skos:definition "Any situation in which a failure of the suspension system is detected. Note: this category excludes failure of the bogie"@en ;
    skos:inScheme iss-sdcr:DirectCauseReportedTypes ;
    skos:notation "B.2.1.5"^^xsd:token ;
    skos:prefLabel "B.2.1.5-Suspension system failure  "@en .

<http://data.europa.eu/949/iss/concepts/safety-direct-cause-reported-types/B.2.2>
    rdf:type skos:Concept ;
    skos:broader <http://data.europa.eu/949/iss/concepts/safety-direct-cause-reported-types/B.2> ;
    skos:definition "A failure of the braking system event falling within the B.2.2 sub-categories for which detailed information is not (yet) available.."@en ;
    skos:inScheme iss-sdcr:DirectCauseReportedTypes ;
    skos:notation "B.2.2"^^xsd:token ;
    skos:prefLabel "B.2.2-Failure of the braking system"@en .

<http://data.europa.eu/949/iss/concepts/safety-direct-cause-reported-types/B.2.2.1>
    rdf:type skos:Concept ;
    skos:broader <http://data.europa.eu/949/iss/concepts/safety-direct-cause-reported-types/B.2.2> ;
    skos:definition "Any situation when the brake system is not operating with in accordance with the planned performance"@en ;
    skos:inScheme iss-sdcr:DirectCauseReportedTypes ;
    skos:notation "B.2.2.1"^^xsd:token ;
    skos:prefLabel "B.2.2.1-Brake not operating with the planned performance   "@en .

<http://data.europa.eu/949/iss/concepts/safety-direct-cause-reported-types/B.2.3>
    rdf:type skos:Concept ;
    skos:broader <http://data.europa.eu/949/iss/concepts/safety-direct-cause-reported-types/B.2> ;
    skos:definition "Other failure of the rolling stock falling within the B.2.0 sub-categories for which detailed information is not (yet) available."@en ;
    skos:inScheme iss-sdcr:DirectCauseReportedTypes ;
    skos:notation "B.2.3"^^xsd:token ;
    skos:prefLabel "B.2.3-Other failures of the rolling stock"@en .

<http://data.europa.eu/949/iss/concepts/safety-direct-cause-reported-types/B.2.3.1>
    rdf:type skos:Concept ;
    skos:broader <http://data.europa.eu/949/iss/concepts/safety-direct-cause-reported-types/B.2.3> ;
    skos:definition "Any technical failure of a signalling system (on-board), resulting in signalling a safety related information less restrictive than that demanded. "@en ;
    skos:inScheme iss-sdcr:DirectCauseReportedTypes ;
    skos:notation "B.2.3.1"^^xsd:token ;
    skos:prefLabel "B.2.3.1-Wrong side signalling (on-board) failure"@en .

<http://data.europa.eu/949/iss/concepts/safety-direct-cause-reported-types/B.2.3.10>
    rdf:type skos:Concept ;
    skos:broader <http://data.europa.eu/949/iss/concepts/safety-direct-cause-reported-types/B.2.3> ;
    skos:definition "Any situation in which the underframe is twisted in excess of the operating design tolerance"@en ;
    skos:inScheme iss-sdcr:DirectCauseReportedTypes ;
    skos:notation "B.2.3.10"^^xsd:token ;
    skos:prefLabel "B.2.3.10-Twisted underframe"@en .

<http://data.europa.eu/949/iss/concepts/safety-direct-cause-reported-types/B.2.3.2>
    rdf:type skos:Concept ;
    skos:broader <http://data.europa.eu/949/iss/concepts/safety-direct-cause-reported-types/B.2.3> ;
    skos:definition "Any technical failure of the on-board system to estimate changes in train position over time"@en ;
    skos:inScheme iss-sdcr:DirectCauseReportedTypes ;
    skos:notation "B.2.3.2"^^xsd:token ;
    skos:prefLabel "B.2.3.2-Odometry error"@en .

<http://data.europa.eu/949/iss/concepts/safety-direct-cause-reported-types/B.2.3.3>
    rdf:type skos:Concept ;
    skos:broader <http://data.europa.eu/949/iss/concepts/safety-direct-cause-reported-types/B.2.3> ;
    skos:definition "Any situation involving a failure of the on-board side of the train detection system"@en ;
    skos:inScheme iss-sdcr:DirectCauseReportedTypes ;
    skos:notation "B.2.3.3"^^xsd:token ;
    skos:prefLabel "B.2.3.3-Train detection equipment failure (on-board)"@en .

<http://data.europa.eu/949/iss/concepts/safety-direct-cause-reported-types/B.2.3.4>
    rdf:type skos:Concept ;
    skos:broader <http://data.europa.eu/949/iss/concepts/safety-direct-cause-reported-types/B.2.3> ;
    skos:definition "Any situation when a rolling stock part detaches and falls on the ground."@en ;
    skos:inScheme iss-sdcr:DirectCauseReportedTypes ;
    skos:notation "B.2.3.4"^^xsd:token ;
    skos:prefLabel "B.2.3.4-Losing of rolling stock parts"@en .

<http://data.europa.eu/949/iss/concepts/safety-direct-cause-reported-types/B.2.3.5>
    rdf:type skos:Concept ;
    skos:broader <http://data.europa.eu/949/iss/concepts/safety-direct-cause-reported-types/B.2.3> ;
    skos:definition "Any situation involving a technical failure of the – electrical motor -  traction"@en ;
    skos:inScheme iss-sdcr:DirectCauseReportedTypes ;
    skos:notation "B.2.3.5"^^xsd:token ;
    skos:prefLabel "B.2.3.5-Traction motor failure (electrical)"@en .

<http://data.europa.eu/949/iss/concepts/safety-direct-cause-reported-types/B.2.3.6>
    rdf:type skos:Concept ;
    skos:broader <http://data.europa.eu/949/iss/concepts/safety-direct-cause-reported-types/B.2.3> ;
    skos:definition "Any situation involving a technical failure of the – diesel engine -  traction"@en ;
    skos:inScheme iss-sdcr:DirectCauseReportedTypes ;
    skos:notation "B.2.3.6"^^xsd:token ;
    skos:prefLabel "B.2.3.6-Diesel engine failure"@en .

<http://data.europa.eu/949/iss/concepts/safety-direct-cause-reported-types/B.2.3.7>
    rdf:type skos:Concept ;
    skos:broader <http://data.europa.eu/949/iss/concepts/safety-direct-cause-reported-types/B.2.3> ;
    skos:definition "Any situation in which the railway vehicles detach as a result of a technical .failure."@en ;
    skos:inScheme iss-sdcr:DirectCauseReportedTypes ;
    skos:notation "B.2.3.7"^^xsd:token ;
    skos:prefLabel "B.2.3.7-Coupling failure"@en .

<http://data.europa.eu/949/iss/concepts/safety-direct-cause-reported-types/B.2.3.8>
    rdf:type skos:Concept ;
    skos:broader <http://data.europa.eu/949/iss/concepts/safety-direct-cause-reported-types/B.2.3> ;
    skos:definition "Any situation involving a technical malfunctioning of the doors"@en ;
    skos:inScheme iss-sdcr:DirectCauseReportedTypes ;
    skos:notation "B.2.3.8"^^xsd:token ;
    skos:prefLabel "B.2.3.8-Doors failure"@en .

<http://data.europa.eu/949/iss/concepts/safety-direct-cause-reported-types/B.2.3.9>
    rdf:type skos:Concept ;
    skos:broader <http://data.europa.eu/949/iss/concepts/safety-direct-cause-reported-types/B.2.3> ;
    skos:definition "Any situation involving a technical malfunctioning of the on-board ventilation system. Note: for example, a loss of ventilation in a train compromising fire management plan, potentially leading to victims or damage"@en ;
    skos:inScheme iss-sdcr:DirectCauseReportedTypes ;
    skos:notation "B.2.3.9"^^xsd:token ;
    skos:prefLabel "B.2.3.9-Loss of ventilation"@en .

<http://data.europa.eu/949/iss/concepts/safety-direct-cause-reported-types/B.3>
    rdf:type skos:Concept ;
    skos:broader <http://data.europa.eu/949/iss/concepts/safety-direct-cause-reported-types/B> ;
    skos:definition "A technical failure of the infrastructure falling within the B.3 sub-categories for which detailed information is not (yet) available."@en ;
    skos:inScheme iss-sdcr:DirectCauseReportedTypes ;
    skos:notation "B.3"^^xsd:token ;
    skos:prefLabel "B.3-Technical Failure of the infrastructure"@en .

<http://data.europa.eu/949/iss/concepts/safety-direct-cause-reported-types/B.3.1>
    rdf:type skos:Concept ;
    skos:broader <http://data.europa.eu/949/iss/concepts/safety-direct-cause-reported-types/B.3> ;
    skos:definition "A failure of the track falling within the B.3.1 sub-categories for which detailed information is not (yet) available."@en ;
    skos:inScheme iss-sdcr:DirectCauseReportedTypes ;
    skos:notation "B.3.1"^^xsd:token ;
    skos:prefLabel "B.3.1-Failure of the track"@en .

<http://data.europa.eu/949/iss/concepts/safety-direct-cause-reported-types/B.3.1.1>
    rdf:type skos:Concept ;
    skos:broader <http://data.europa.eu/949/iss/concepts/safety-direct-cause-reported-types/B.3.1> ;
    skos:definition "Any rail which is separated in two or more pieces, or any rail from which a piece of metal becomes detached, causing a gap of more than 50 mm in length and more than 10 mm in depth on the running surface."@en ;
    skos:inScheme iss-sdcr:DirectCauseReportedTypes ;
    skos:notation "B.3.1.1"^^xsd:token ;
    skos:prefLabel "B.3.1.1-Broken rail"@en .

<http://data.europa.eu/949/iss/concepts/safety-direct-cause-reported-types/B.3.1.2>
    rdf:type skos:Concept ;
    skos:broader <http://data.europa.eu/949/iss/concepts/safety-direct-cause-reported-types/B.3.1> ;
    skos:definition "Any fault related to the continuum and the geometry of track, requiring track to be placed out of service or immediate restriction of permitted speed"@en ;
    skos:inScheme iss-sdcr:DirectCauseReportedTypes ;
    skos:notation "B.3.1.2"^^xsd:token ;
    skos:prefLabel "B.3.1.2-Track buckle and other track misalignment"@en .

<http://data.europa.eu/949/iss/concepts/safety-direct-cause-reported-types/B.3.1.2.1>
    rdf:type skos:Concept ;
    skos:broader <http://data.europa.eu/949/iss/concepts/safety-direct-cause-reported-types/B.3.1.2> ;
    skos:definition "Any situation in which the gauge spread is outside of the accepted tolerance"@en ;
    skos:inScheme iss-sdcr:DirectCauseReportedTypes ;
    skos:notation "B.3.1.2.1"^^xsd:token ;
    skos:prefLabel "B.3.1.2.1-Gauge spread"@en .

<http://data.europa.eu/949/iss/concepts/safety-direct-cause-reported-types/B.3.1.2.2>
    rdf:type skos:Concept ;
    skos:broader <http://data.europa.eu/949/iss/concepts/safety-direct-cause-reported-types/B.3.1.2> ;
    skos:definition "Any situation in which the track twist is outside of the accepted tolerance"@en ;
    skos:inScheme iss-sdcr:DirectCauseReportedTypes ;
    skos:notation "B.3.1.2.2"^^xsd:token ;
    skos:prefLabel "B.3.1.2.2-Track twist"@en .

<http://data.europa.eu/949/iss/concepts/safety-direct-cause-reported-types/B.3.1.2.3>
    rdf:type skos:Concept ;
    skos:broader <http://data.europa.eu/949/iss/concepts/safety-direct-cause-reported-types/B.3.1.2> ;
    skos:definition "Any situation in which the rail fastening or joint is outside of the accepted tolerance"@en ;
    skos:inScheme iss-sdcr:DirectCauseReportedTypes ;
    skos:notation "B.3.1.2.3"^^xsd:token ;
    skos:prefLabel "B.3.1.2.3-Improper rail fastening and joints"@en .

<http://data.europa.eu/949/iss/concepts/safety-direct-cause-reported-types/B.3.1.3>
    rdf:type skos:Concept ;
    skos:broader <http://data.europa.eu/949/iss/concepts/safety-direct-cause-reported-types/B.3.1> ;
    skos:definition "Any technical failure of a signalling system (infrastructure), resulting in signalling safety related information less restrictive than that demanded. "@en ;
    skos:inScheme iss-sdcr:DirectCauseReportedTypes ;
    skos:notation "B.3.1.3"^^xsd:token ;
    skos:prefLabel "B.3.1.3-Wrong side signalling (infrastructure) failure"@en .

<http://data.europa.eu/949/iss/concepts/safety-direct-cause-reported-types/B.3.1.4>
    rdf:type skos:Concept ;
    skos:broader <http://data.europa.eu/949/iss/concepts/safety-direct-cause-reported-types/B.3.1> ;
    skos:definition "Any situation in which a switch or a crossing is not operating as expected"@en ;
    skos:inScheme iss-sdcr:DirectCauseReportedTypes ;
    skos:notation "B.3.1.4"^^xsd:token ;
    skos:prefLabel "B.3.1.4-Switch and crossing failure"@en .

<http://data.europa.eu/949/iss/concepts/safety-direct-cause-reported-types/B.3.1.5>
    rdf:type skos:Concept ;
    skos:broader <http://data.europa.eu/949/iss/concepts/safety-direct-cause-reported-types/B.3.1> ;
    skos:definition "Any occasion when a train or rail vehicle passes over a level crossing with lower protection level than required."@en ;
    skos:inScheme iss-sdcr:DirectCauseReportedTypes ;
    skos:notation "B.3.1.5"^^xsd:token ;
    skos:prefLabel "B.3.1.5-Failure of the level crossing equipment"@en .

<http://data.europa.eu/949/iss/concepts/safety-direct-cause-reported-types/B.3.2>
    rdf:type skos:Concept ;
    skos:broader <http://data.europa.eu/949/iss/concepts/safety-direct-cause-reported-types/B.3> ;
    skos:definition "A structures failure event falling within the B.3.2 sub-categories for which detailed information is not (yet) available."@en ;
    skos:inScheme iss-sdcr:DirectCauseReportedTypes ;
    skos:notation "B.3.2"^^xsd:token ;
    skos:prefLabel "B.3.2-Structures failure"@en .

<http://data.europa.eu/949/iss/concepts/safety-direct-cause-reported-types/B.3.2.1>
    rdf:type skos:Concept ;
    skos:broader <http://data.europa.eu/949/iss/concepts/safety-direct-cause-reported-types/B.3.2> ;
    skos:definition "Any situation in which a tunnel structure is not operating as expected"@en ;
    skos:inScheme iss-sdcr:DirectCauseReportedTypes ;
    skos:notation "B.3.2.1"^^xsd:token ;
    skos:prefLabel "B.3.2.1-Tunnel failure"@en .

<http://data.europa.eu/949/iss/concepts/safety-direct-cause-reported-types/B.3.2.2>
    rdf:type skos:Concept ;
    skos:broader <http://data.europa.eu/949/iss/concepts/safety-direct-cause-reported-types/B.3.2> ;
    skos:definition "Any situation in which a viaduct structure is not operating as expected"@en ;
    skos:inScheme iss-sdcr:DirectCauseReportedTypes ;
    skos:notation "B.3.2.2"^^xsd:token ;
    skos:prefLabel "B.3.2.2-Viaduct failure"@en .

<http://data.europa.eu/949/iss/concepts/safety-direct-cause-reported-types/B.3.2.3>
    rdf:type skos:Concept ;
    skos:broader <http://data.europa.eu/949/iss/concepts/safety-direct-cause-reported-types/B.3.2> ;
    skos:definition "Any situation in which a culvert structure is not operating as expected"@en ;
    skos:inScheme iss-sdcr:DirectCauseReportedTypes ;
    skos:notation "B.3.2.3"^^xsd:token ;
    skos:prefLabel "B.3.2.3-Culvert failures"@en .

<http://data.europa.eu/949/iss/concepts/safety-direct-cause-reported-types/B.3.2.4>
    rdf:type skos:Concept ;
    skos:broader <http://data.europa.eu/949/iss/concepts/safety-direct-cause-reported-types/B.3.2> ;
    skos:definition "Any situation in which a rail bridge structure is not operating as expected"@en ;
    skos:inScheme iss-sdcr:DirectCauseReportedTypes ;
    skos:notation "B.3.2.4"^^xsd:token ;
    skos:prefLabel "B.3.2.4-Rail bridge structural failure"@en .

<http://data.europa.eu/949/iss/concepts/safety-direct-cause-reported-types/B.3.2.5>
    rdf:type skos:Concept ;
    skos:broader <http://data.europa.eu/949/iss/concepts/safety-direct-cause-reported-types/B.3.2> ;
    skos:definition "Any situation in which an over line bridge structure is not operating as expected"@en ;
    skos:inScheme iss-sdcr:DirectCauseReportedTypes ;
    skos:notation "B.3.2.5"^^xsd:token ;
    skos:prefLabel "B.3.2.5-Over line bridge (e.g. pedestrian) failure"@en .

<http://data.europa.eu/949/iss/concepts/safety-direct-cause-reported-types/B.3.2.6>
    rdf:type skos:Concept ;
    skos:broader <http://data.europa.eu/949/iss/concepts/safety-direct-cause-reported-types/B.3.2> ;
    skos:definition "Any situation in which a station structure is not operating as expected"@en ;
    skos:inScheme iss-sdcr:DirectCauseReportedTypes ;
    skos:notation "B.3.2.6"^^xsd:token ;
    skos:prefLabel "B.3.2.6-Station (building) Structure failure"@en .

<http://data.europa.eu/949/iss/concepts/safety-direct-cause-reported-types/B.3.2.7>
    rdf:type skos:Concept ;
    skos:broader <http://data.europa.eu/949/iss/concepts/safety-direct-cause-reported-types/B.3.2> ;
    skos:definition "Any situation in which a platform structure is not operating as expected"@en ;
    skos:inScheme iss-sdcr:DirectCauseReportedTypes ;
    skos:notation "B.3.2.7"^^xsd:token ;
    skos:prefLabel "B.3.2.7-Platform failure"@en .

<http://data.europa.eu/949/iss/concepts/safety-direct-cause-reported-types/B.3.2.8>
    rdf:type skos:Concept ;
    skos:broader <http://data.europa.eu/949/iss/concepts/safety-direct-cause-reported-types/B.3.2> ;
    skos:definition "Any situation in which a earthwork/embankment structure is not operating as expected"@en ;
    skos:inScheme iss-sdcr:DirectCauseReportedTypes ;
    skos:notation "B.3.2.8"^^xsd:token ;
    skos:prefLabel "B.3.2.8-Disorder of earthworks/embankment failure"@en .

<http://data.europa.eu/949/iss/concepts/safety-direct-cause-reported-types/B.3.3>
    rdf:type skos:Concept ;
    skos:broader <http://data.europa.eu/949/iss/concepts/safety-direct-cause-reported-types/B.3> ;
    skos:definition "Other failure of the infrastructure falling within the B.3.3 sub-categories for which detailed information is not (yet) available."@en ;
    skos:inScheme iss-sdcr:DirectCauseReportedTypes ;
    skos:notation "B.3.3"^^xsd:token ;
    skos:prefLabel "B.3.3-Other failures of the infrastructure"@en .

<http://data.europa.eu/949/iss/concepts/safety-direct-cause-reported-types/B.3.3.1>
    rdf:type skos:Concept ;
    skos:broader <http://data.europa.eu/949/iss/concepts/safety-direct-cause-reported-types/B.3.3> ;
    skos:definition "Any situation in which a power supply equipment is not operating as expected"@en ;
    skos:inScheme iss-sdcr:DirectCauseReportedTypes ;
    skos:notation "B.3.3.1"^^xsd:token ;
    skos:prefLabel "B.3.3.1-Power supply equipment failure"@en .

<http://data.europa.eu/949/iss/concepts/safety-direct-cause-reported-types/B.3.3.2>
    rdf:type skos:Concept ;
    skos:broader <http://data.europa.eu/949/iss/concepts/safety-direct-cause-reported-types/B.3.3> ;
    skos:definition "Any situation in which a – track side – train detection equipment is not operating as expected "@en ;
    skos:inScheme iss-sdcr:DirectCauseReportedTypes ;
    skos:notation "B.3.3.2"^^xsd:token ;
    skos:prefLabel "B.3.3.2-Train detection equipment failure (trackside)"@en .

<http://data.europa.eu/949/iss/concepts/safety-direct-cause-reported-types/B.3.3.3>
    rdf:type skos:Concept ;
    skos:broader <http://data.europa.eu/949/iss/concepts/safety-direct-cause-reported-types/B.3.3> ;
    skos:definition "Any situation in which an overhead contact line is not operating as expected"@en ;
    skos:inScheme iss-sdcr:DirectCauseReportedTypes ;
    skos:notation "B.3.3.3"^^xsd:token ;
    skos:prefLabel "B.3.3.3-Overhead contact line failure"@en .

<http://data.europa.eu/949/iss/concepts/safety-direct-cause-reported-types/B.3.3.4>
    rdf:type skos:Concept ;
    skos:broader <http://data.europa.eu/949/iss/concepts/safety-direct-cause-reported-types/B.3.3> ;
    skos:definition "Any situation involving a technical malfunctioning of the ventilation system in a tunnel or in a station. Note: for example, a loss of tunnel ventilation compromising fire management plan, potentially leading to victims or damage"@en ;
    skos:inScheme iss-sdcr:DirectCauseReportedTypes ;
    skos:notation "B.3.3.4"^^xsd:token ;
    skos:prefLabel "B.3.3.4-Loss of ventilation"@en .

<http://data.europa.eu/949/iss/concepts/safety-direct-cause-reported-types/B.4>
    rdf:type skos:Concept ;
    skos:broader <http://data.europa.eu/949/iss/concepts/safety-direct-cause-reported-types/B> ;
    skos:definition "Other category B event falling within the B.4 sub-categories for which detailed information is not (yet) available"@en ;
    skos:inScheme iss-sdcr:DirectCauseReportedTypes ;
    skos:notation "B.4"^^xsd:token ;
    skos:prefLabel "B.4-Other category B event types"@en .

<http://data.europa.eu/949/iss/concepts/safety-direct-cause-reported-types/B.4.1>
    rdf:type skos:Concept ;
    skos:broader <http://data.europa.eu/949/iss/concepts/safety-direct-cause-reported-types/B.4> ;
    skos:definition "Any occasion in which a fire is taking place in proximity of rail infrastructure, affecting the integrity of the infrastructure or the operations."@en ;
    skos:inScheme iss-sdcr:DirectCauseReportedTypes ;
    skos:notation "B.4.1"^^xsd:token ;
    skos:prefLabel "B.4.1-Fire in proximity of rail infrastructure "@en .

<http://data.europa.eu/949/iss/concepts/safety-direct-cause-reported-types/B.4.2>
    rdf:type skos:Concept ;
    skos:broader <http://data.europa.eu/949/iss/concepts/safety-direct-cause-reported-types/B.4> ;
    skos:definition "Any occasion in which the unauthorised presence of staff/employees (i.e. not in accordance with the applicable requirements) is detected. This also includes sub-contractor staff."@en ;
    skos:inScheme iss-sdcr:DirectCauseReportedTypes ;
    skos:notation "B.4.2"^^xsd:token ;
    skos:prefLabel "B.4.2-Unauthorised presence of staff/employees on railway system"@en .

<http://data.europa.eu/949/iss/concepts/safety-direct-cause-reported-types/B.4.3>
    rdf:type skos:Concept ;
    skos:broader <http://data.europa.eu/949/iss/concepts/safety-direct-cause-reported-types/B.4> ;
    skos:definition "Any occasion in which the unauthorised presence of third parties on the railway system (i.e. not in accordance with the applicable requirements) is detected. "@en ;
    skos:inScheme iss-sdcr:DirectCauseReportedTypes ;
    skos:notation "B.4.3"^^xsd:token ;
    skos:prefLabel "B.4.3-Unauthorised presence of other third parties on the railway system "@en .

<http://data.europa.eu/949/iss/concepts/safety-direct-cause-reported-types/B.4.4>
    rdf:type skos:Concept ;
    skos:broader <http://data.europa.eu/949/iss/concepts/safety-direct-cause-reported-types/B.4> ;
    skos:definition "Any occasion in which the improper or incautious use by persons of authorised passages between platforms in the stations is detected"@en ;
    skos:inScheme iss-sdcr:DirectCauseReportedTypes ;
    skos:notation "B.4.4"^^xsd:token ;
    skos:prefLabel "B.4.4-Improper or incautious use of authorised passages between platforms in the stations"@en .

<http://data.europa.eu/949/iss/concepts/safety-direct-cause-reported-types/B.4.5>
    rdf:type skos:Concept ;
    skos:broader <http://data.europa.eu/949/iss/concepts/safety-direct-cause-reported-types/B.4> ;
    skos:definition "Any incident involving dangerous goods to be reported in accordance with section 1.8.5 of ‘RID’ (as referred to in Annex II.1 to Directive 2008/68/EC, as amended) and not covered by another type B event."@en ;
    skos:inScheme iss-sdcr:DirectCauseReportedTypes ;
    skos:notation "B.4.5"^^xsd:token ;
    skos:prefLabel "B.4.5-Dangerous goods incidents not related to another type B event"@en .

