    @prefix rdf: <http://www.w3.org/1999/02/22-rdf-syntax-ns#> .
@prefix rdfs: <http://www.w3.org/2000/01/rdf-schema#> .
@prefix owl: <http://www.w3.org/2002/07/owl#> .
@prefix xsd: <http://www.w3.org/2001/XMLSchema#> .
@prefix dct: <http://purl.org/dc/terms/> .
@prefix skos: <http://www.w3.org/2004/02/skos/core#> .
@prefix cc: <http://creativecommons.org/ns#> .

@prefix iss-cf: <http://data.europa.eu/949/iss/concepts/contributing-factors/> .





#################################################################
#
#    Concept Schemes
#
#################################################################



iss-cf:ContributingFactors a skos:ConceptScheme ; 
    dct:issued "2024-08-29"^^xsd:date ;
    dct:modified "2025-05-25"^^xsd:date ;
    skos:changeNote "Updates with latest values"@en ;
    cc:license <https://creativecommons.org/licenses/by/4.0/> ;
    rdfs:comment "Controlled SKOS-based vocabulary defined by the European Union Agency for Railways to describe concepts related to the Information Sharing System (ISS) in accordance with the draft delegated act of the future CSM ASLP Regulation."@en ;
    rdfs:label "Contributing Conditions"@en ;
    skos:hasTopConcept iss-cf:CF.0, iss-cf:CF.1 ;
    skos:prefLabel "Contributing Factors"@en ;
    dct:title "Concept scheme grouping contributing factors that affect an occurrence"@en .



#################################################################
#
#    Concept instances
#
#################################################################

iss-cf:CF.0	a skos:Concept ;
	skos:prefLabel "Other contributing factors"@en ;
	skos:definition "Any other contributing factor not covered by any of the category or sub-categories coded above. A reporting of information in accordance with section 3.3 of Appendix A - Part C shall apply."@en ;
	skos:notation "CF.0"^^xsd:token ;
	skos:topConceptOf iss-cf:ContributingFactors ;
	skos:inScheme iss-cf:ContributingFactors ;
	.

iss-cf:CF.1 a skos:Concept ;
	skos:prefLabel "Performance relevant factor"@en ;
	skos:definition "Performance relevant factor"@en ;
	skos:notation "CF.1"^^xsd:token;
	skos:topConceptOf iss-cf:ContributingFactors ;
	skos:inScheme iss-cf:ContributingFactors ;
	.

iss-cf:CF.1.1.0 a skos:Concept;
  skos:broader iss-cf:CF.1.1;
  skos:definition "Any contributing factor falling within the category ‘Dynamic situational factors’, but not covered by any of the sub-categories coded above. A reporting of information in accordance with section 3.3 of Appendix A - Part C shall apply."@en;
  skos:inScheme iss-cf:ContributingFactors;
  skos:notation "CF.1.1.0"^^xsd:token;
  skos:prefLabel "Other dynamic situational factors"@en .

iss-cf:CF.1.1.1 a skos:Concept;
  skos:broader iss-cf:CF.1.1;
  skos:definition "Refers to two different aspects of the time available (both real or perceived): the pressure generated by uncertainties, changes and the results to be achieved sometimes on competing objectives; and the pressure generated by the time available to analyse, anticipate, coordinate, communicate decide, act or react, check, report, etc."@en;
  skos:inScheme iss-cf:ContributingFactors;
  skos:notation "CF.1.1.1"^^xsd:token;
  skos:prefLabel "Pressure "@en .

iss-cf:CF.1.1.2 a skos:Concept;
  skos:broader iss-cf:CF.1.1;
  skos:definition "Refers to two different aspects of the complexity of the situation. First, it refers to the amount and ambiguity of information and its timing, the interacting activities and actors, and their dynamic evolution from one moment to another, forcing the update or refresh of the memory. Second, it refers to the autonomy left in controlling the situation, in making decisions, in carrying out actions and recovering them, with the eventual delays, before their consequences and their visibility."@en;
  skos:inScheme iss-cf:ContributingFactors;
  skos:notation "CF.1.1.2"^^xsd:token;
  skos:prefLabel "Complexity"@en .

iss-cf:CF.1.1.3 a skos:Concept;
  skos:broader iss-cf:CF.1.1;
  skos:definition "Refers to two different aspects of the monotony within situations. Firstly, the repetition of the situation, and the habit of acting or thinking in a particular way (more mechanical, more automatic). Secondly, boredom due to lack of change in the environment. Both situations induce a challenge to get out of the largely dominant work logic at the right time, and to act differently, considering elements that are maybe rarer or surprising, and somehow temporarily undetected. Because of boredom or repetition, thoughts may deviate from the situation being treated more automatically and may need more time to adapt to change."@en;
  skos:inScheme iss-cf:ContributingFactors;
  skos:notation "CF.1.1.3"^^xsd:token;
  skos:prefLabel "Monotony "@en .

iss-cf:CF.1.1.4 a skos:Concept;
  skos:broader iss-cf:CF.1.1;
  skos:definition "Refers to the hours or periods of work actually worked with two aspects: the distribution of physical and mental workloads during these periods of work (quality and quantity of the work repartition within the time of work); and, the sequence of the actual work periods, with beginning and end time, the effective breaks, organised in 1/2/3 teams over 24 hours and during the last 3 weeks to 3 months (quality of the work shifts or patterns as experienced by the individuals)."@en;
  skos:inScheme iss-cf:ContributingFactors;
  skos:notation "CF.1.1.4"^^xsd:token;
  skos:prefLabel "Work-rhythms "@en .

iss-cf:CF.1.1.5 a skos:Concept;
  skos:broader iss-cf:CF.1.1;
  skos:definition "Refers to the temporary physical characteristics of the workplace that can have an influence on the physical, mental and emotional state of the worker, including cognitive and social activities in general. It relates to e.g.: visibility and light, noise, vibrations, accessibility, working positions, static and dynamic physical loads, distances to be covered, and variable weather conditions; as they interact with railways activities or decision-making processes."@en;
  skos:inScheme iss-cf:ContributingFactors;
  skos:notation "CF.1.1.5"^^xsd:token;
  skos:prefLabel "Environment "@en .

iss-cf:CF.1.2.0 a skos:Concept;
  skos:broader iss-cf:CF.1.2;
  skos:definition "Any contributing factor falling within the category ‘Dynamic staff factors’, but not covered by any of the sub-categories coded above. A reporting of information in accordance with section 3.3 of Appendix A - Part C shall apply."@en;
  skos:inScheme iss-cf:ContributingFactors;
  skos:notation "CF.1.2.0"^^xsd:token;
  skos:prefLabel "Other dynamic staff factors"@en .

iss-cf:CF.1.2.1 a skos:Concept;
  skos:broader iss-cf:CF.1.2;
  skos:definition "Refers to the persons’ intentions which in the situation guide them to decide and act as they do. It covers three aspects: the intention before and during the actions (for which purpose they do what they do); the reasoning in a situation (taking into account how the persons considered the situation at the action time or just before); and when useful, the categorisation of the type of variability or deviation from the intended action (e.g. involuntary – voluntary, positive – negative, type of error, type of violation)."@en;
  skos:inScheme iss-cf:ContributingFactors;
  skos:notation "CF.1.2.1"^^xsd:token;
  skos:prefLabel "Intentions "@en .

iss-cf:CF.1.2.2 a skos:Concept;
  skos:broader iss-cf:CF.1.2;
  skos:definition "Refers to two aspects that create the conditions for concentration: an external one that regards the different professional activities that influence the capacity for attention because they force this capacity to be divided and therefore reduced; and, an internal one that is more psychological or personal because the flow of thoughts can split the capacity of attention between what or why to do, how to do, when to do and other professional or personal life thoughts."@en;
  skos:inScheme iss-cf:ContributingFactors;
  skos:notation "CF.1.2.2"^^xsd:token;
  skos:prefLabel "Attention "@en .

iss-cf:CF.1.2.3 a skos:Concept;
  skos:broader iss-cf:CF.1.2;
  skos:definition "Refers to sleep-related fatigue (in quality, in quantity, at night-time), regardless of the reasons, which is a temporary state that can lead to variations in behaviour or decisions, i.e. deviation, error or violation, e.g. due to missed information, inadequate analysis or unanticipated action. Fatigue is a decreased capacity to perform mental or physical work, with involuntary physiological performance decrements (e.g. hypo-vigilance, micro-sleeps), mood disorders and cognitive impairment, due to inadequate restorative sleep, time of day, length of the waking period, or due to the interaction between the lack of breaks and some characteristics of the activities, etc."@en;
  skos:inScheme iss-cf:ContributingFactors;
  skos:notation "CF.1.2.3"^^xsd:token;
  skos:prefLabel "Fatigue"@en .

iss-cf:CF.1.2.4 a skos:Concept;
  skos:broader iss-cf:CF.1.2;
  skos:definition "Refers to specific emotions, due to chronic or shocking stimulation and, in its basic meaning, to any type of change that causes physical, emotional or psychological strain. A common reference situation for stress is when staff (individuals, groups) feel an imbalance between what they are asked to do professionally and the resources they have to do it (time, instructions, skills, support, tools, etc.)."@en;
  skos:inScheme iss-cf:ContributingFactors;
  skos:notation "CF.1.2.4"^^xsd:token;
  skos:prefLabel "Stress "@en .

iss-cf:CF.1.2.5 a skos:Concept;
  skos:broader iss-cf:CF.1.2;
  skos:definition "Refers to both situational awareness and self-awareness. This factor covers the three stages of situational awareness: perception of information, understanding of what is perceived, and projection of how to react on the basis of the perceptions and their understood meaning (including risks). This factor also covers self-awareness: of a person’s own state of mind and health, of a person’s own limitations, of a person’s own past decisions and actions, as well as their past outcomes and (risk of) consequences."@en;
  skos:inScheme iss-cf:ContributingFactors;
  skos:notation "CF.1.2.5"^^xsd:token;
  skos:prefLabel "Awareness"@en .

iss-cf:CF.1.3.0 a skos:Concept;
  skos:broader iss-cf:CF.1.3;
  skos:definition "Any contributing factor falling within the category ‘Static situational factors’, but not covered by any of the sub-categories coded above. A reporting of information in accordance with section 3.3 of Appendix A - Part C shall apply."@en;
  skos:inScheme iss-cf:ContributingFactors;
  skos:notation "CF.1.3.0"^^xsd:token;
  skos:prefLabel "Other static situational factors"@en .

iss-cf:CF.1.3.1 a skos:Concept;
  skos:broader iss-cf:CF.1.3;
  skos:definition "Refers to the relative end-user-based approach when designing or changing procedures and instructions, tools and equipment (incl. human-machine/computer interfaces), processes and the levels of automation in them. This requires the definition of the user-experience view and use of what is to be designed or modified, considering tasks allocation, workload fluctuation, interactions between humans to be defined - and with the IT interfaces, anticipated variabilities (deviations, errors, etc.) and their consequences, residual risks left to end-users, levels of autonomy, the remaining purpose of the work when reduced or automated, etc."@en;
  skos:inScheme iss-cf:ContributingFactors;
  skos:notation "CF.1.3.1"^^xsd:token;
  skos:prefLabel "Design "@en .

iss-cf:CF.1.3.2 a skos:Concept;
  skos:broader iss-cf:CF.1.3;
  skos:definition "Refers to the directives and regulations from all levels, and the rules, procedures, and instructions produced for a standardised performance of all the tasks (in a broad sense). This includes not only their existence (or not) and availability, but also their quality to enable the work to be carried out properly (e.g. resources defined) while controlling the related risks. This factor also covers the interactions between tasks, and with other processes (e.g. monitoring)."@en;
  skos:inScheme iss-cf:ContributingFactors;
  skos:notation "CF.1.3.2"^^xsd:token;
  skos:prefLabel "Instructions "@en .

iss-cf:CF.1.3.5 a skos:Concept;
  skos:broader iss-cf:CF.1.3;
  skos:definition "Refers to the influences the societal and institutional contexts may have on the staff concerned (staff and leaders) and their work situations (incl. projects, resources and budgets, etc.). This covers the influences of the regulation of the sector (national, EU), the influences of the economy, politics, media, and of the societal events (sabotage, terrorism, social climate, security climate, health crisis, etc.)."@en;
  skos:inScheme iss-cf:ContributingFactors;
  skos:notation "CF.1.3.5"^^xsd:token;
  skos:prefLabel "Context"@en .

iss-cf:CF.1.4.0 a skos:Concept;
  skos:broader iss-cf:CF.1.4;
  skos:definition "Any contributing factor falling within the category ‘Static staff factors’, but not covered by any of the sub-categories coded above. A reporting of information in accordance with section 3.3 of Appendix A - Part C shall apply."@en;
  skos:inScheme iss-cf:ContributingFactors;
  skos:notation "CF.1.4.0"^^xsd:token;
  skos:prefLabel "Other static staff factors"@en .

iss-cf:CF.1.4.1 a skos:Concept;
  skos:broader iss-cf:CF.1.4;
  skos:definition "Refers primarily to levels of familiarity with the activities and of specific working conditions (in a broad sense), which also provide implicit knowledge and/or incidental learning. Expertise can sometimes be detrimental, e.g. after introduction of changes or the occurrence of less practiced patterns. Beginners may need years of varied practice before they are comfortable with more difficult or rare cases. Also refers to career paths linked to varied work activities or circumstances or diversified tools, which career paths provide a wider range of practices."@en;
  skos:inScheme iss-cf:ContributingFactors;
  skos:notation "CF.1.4.1"^^xsd:token;
  skos:prefLabel "Experience"@en .

iss-cf:CF.1.4.2 a skos:Concept;
  skos:broader iss-cf:CF.1.4;
  skos:definition "Refers to the psychological and physiological characteristics of the concerned staff, including health. This includes psychological attitudes that influence behaviour at work such as self-confidence, openness to experience, conscientiousness, extraversion, agreeableness, emotional stability. Health criteria can also be linked with aging, physiological needs or evolving characteristics. It also includes the necessary periodic checks and monitoring of the relevant personal characteristics for safety, depending on the person’s responsibilities.  "@en;
  skos:inScheme iss-cf:ContributingFactors;
  skos:notation "CF.1.4.2"^^xsd:token;
  skos:prefLabel "Personal"@en .

iss-cf:CF.1.4.3 a skos:Concept;
  skos:broader iss-cf:CF.1.4;
  skos:definition "Refers to the commitment and adherence of the concerned staff to the company's objectives, values and priorities. It also refers to motivation management, and to the balance between extrinsic (salaries, bonuses, pressure, etc.) and intrinsic (fulfilment, autonomy, challenge, etc.) type of motivation. Specific to safety, it also refers to the task’s important rules and how they make sense, and to the way the organisation manages risks, changes, improvements; and communicates on them."@en;
  skos:inScheme iss-cf:ContributingFactors;
  skos:notation "CF.1.4.3"^^xsd:token;
  skos:prefLabel "Motivation "@en .

iss-cf:CF.1.4.4 a skos:Concept;
  skos:broader iss-cf:CF.1.4;
  skos:definition "Refers to the point at which staff concerned meets the requirements of the roles, activities, responsibilities and situations to be managed, in terms of qualifications and competencies (attitudes, awareness, knowledge, skills, including non-technical skills) as demonstrated during the review sessions, adjustments and periodic checks. Sufficient is not always enough: sometimes assessed out of context, theoretical questions–answers are not sufficiently broad, diverse or practical to prepare for dangerous or rare or unregulated situations."@en;
  skos:inScheme iss-cf:ContributingFactors;
  skos:notation "CF.1.4.4"^^xsd:token;
  skos:prefLabel "Competencies"@en .

iss-cf:CF.1.4.5 a skos:Concept;
  skos:broader iss-cf:CF.1.4;
  skos:definition "Refers to the capability to make decisions based on information, its interpretation, the context, the nature of the issue to solve: e.g. ability to interpret situations, quality of memory processes, tendency to follow more or less the procedures or to reconsider the competing objectives, ability to be creative, tendency to be of service for others, or ability to interact with others about the decision-making process, etc.."@en;
  skos:inScheme iss-cf:ContributingFactors;
  skos:notation "CF.1.4.5"^^xsd:token;
  skos:prefLabel "Decision-making "@en .

iss-cf:CF.1.5.0 a skos:Concept;
  skos:broader iss-cf:CF.1.5;
  skos:definition "Any contributing factor falling within the category ‘Relation factors’, but not covered by any of the sub-categories coded above. A reporting of information in accordance with section 3.3 of Appendix A - Part C shall apply."@en;
  skos:inScheme iss-cf:ContributingFactors;
  skos:notation "CF.1.5.0"^^xsd:token;
  skos:prefLabel "Other relational factors"@en .

iss-cf:CF.1.5.1 a skos:Concept;
  skos:broader iss-cf:CF.1.5;
  skos:definition "Refers to the message and content of the communication, the way in which the interlocutors understand each other and coordinate to reach an efficient level of communication: it can be between staff members within a team, between teams, with or between contractors, with or between the line manager(s), etc.."@en;
  skos:inScheme iss-cf:ContributingFactors;
  skos:notation "CF.1.5.1"^^xsd:token;
  skos:prefLabel "Communication "@en .

iss-cf:CF.1.5.2 a skos:Concept;
  skos:broader iss-cf:CF.1.5;
  skos:definition "Refers to the management of the power dynamics inherent in any social relationship between people organised in small or larger groups, in particular with issues or influences from: sharing resources, achieving opposing objectives, competing for promotion or career management (with some detrimental effect on individuals and on processes, e.g. hidden agendas or issues, pressure to achieve personal goals). It also refers to the influential relationship to one's own leaders as well as with own collaborators if any."@en;
  skos:inScheme iss-cf:ContributingFactors;
  skos:notation "CF.1.5.2"^^xsd:token;
  skos:prefLabel "Relationships "@en .

iss-cf:CF.1.5.3 a skos:Concept;
  skos:broader iss-cf:CF.1.5;
  skos:definition "Refers to the level of (reciprocal) confidence with which the staff concerned (individuals or groups) can rely on colleagues and on management, and on rules, procedures, and also on technical means such as the (partially) automated tools... in order to carry out their tasks, produce an efficient activity, while fully assuming their responsibilities; even when a failure or an improvement area appears or is to be reported or raised, being sure to be treated fairly."@en;
  skos:inScheme iss-cf:ContributingFactors;
  skos:notation "CF.1.5.3"^^xsd:token;
  skos:prefLabel "Trust "@en .

iss-cf:CF.1.5.4 a skos:Concept;
  skos:broader iss-cf:CF.1.5;
  skos:definition "Refers to anything that strengthens (positively or negatively) professional practices, particularly in relation to safety. Taking the example of a given behaviour: positive reinforcement increases its probability of occurrence; negative reinforcement decreases it. This may be through the presence or absence of feedback or examples (especially the feedback or examples given by managers or instructors, intentionally or not). They can also be incentives or promotion, on the contrary, threats of sanctions or of non-promotion. It can even be about the choice of words, of messages, in official or unofficial communications. And it may concern a wide range of behaviours, referring to past variabilities, to habitual or tolerated deviations, to well-known residual risks, to weak or good monitoring or reporting, etc."@en;
  skos:inScheme iss-cf:ContributingFactors;
  skos:notation "CF.1.5.4"^^xsd:token;
  skos:prefLabel "Reinforcement"@en .

iss-cf:CF.1.5.5 a skos:Concept;
  skos:broader iss-cf:CF.1.5;
  skos:definition "Refers to the consultation and the participation of staff in decision-making processes. It includes the involvement, the inclusion of staff throughout the organisation, for example in projects, actions or meetings. It is about how the organisation involves end-users and their representatives in reviewing or monitoring safety processes and in their continuous improvement."@en;
  skos:inScheme iss-cf:ContributingFactors;
  skos:notation "CF.1.5.5"^^xsd:token;
  skos:prefLabel "Involvement "@en .

iss-cf:CF.1.3 a skos:Concept;
  skos:broader iss-cf:CF.1;
  skos:definition "Lasting characteristics or repetitive elements of a situation that can influence the individuals and the teams or the course of the situation."@en;
  skos:inScheme iss-cf:ContributingFactors;
  skos:notation "CF.1.3"^^xsd:token;
  skos:prefLabel "Static situational factors"@en .

iss-cf:CF.1.1 a skos:Concept;
  skos:broader iss-cf:CF.1;
  skos:definition "Temporary or very short-term characteristics of the situation that can influence individuals and the teams or the course of the situation."@en;
  skos:inScheme iss-cf:ContributingFactors;
  skos:notation "CF.1.1"^^xsd:token;
  skos:prefLabel "Dynamic situational factors"@en .

iss-cf:CF.1.2 a skos:Concept;
  skos:broader iss-cf:CF.1;
  skos:definition "Temporary or very short-term characteristics of individuals and teams that can influence the course of the situation or other concerned staff."@en;
  skos:inScheme iss-cf:ContributingFactors;
  skos:notation "CF.1.2"^^xsd:token;
  skos:prefLabel "Dynamic staff factors"@en .

iss-cf:CF.1.4 a skos:Concept;
  skos:broader iss-cf:CF.1;
  skos:definition "Lasting characteristics or repetitive elements in the concerned individuals and teams that can influence the course of the situation or other concerned staff."@en;
  skos:inScheme iss-cf:ContributingFactors;
  skos:notation "CF.1.4"^^xsd:token;
  skos:prefLabel "Static staff factors"@en .

iss-cf:CF.1.5 a skos:Concept;
  skos:broader iss-cf:CF.1;
  skos:definition "Relational factors between the concerned staff, or between several concerned groups of staff (incl. hierarchy levels), which can influence the course of the situation, or influence the people themselves in their reactions, attitudes, beliefs and perceptions."@en;
  skos:inScheme iss-cf:ContributingFactors;
  skos:notation "CF.1.5"^^xsd:token;
  skos:prefLabel "Relational factors"@en .
