@prefix cc: <http://creativecommons.org/ns#> .
@prefix iss-spae: <http://data.europa.eu/949/iss/concepts/safety-performance-assessment-elements/> .
@prefix dct: <http://purl.org/dc/terms/> .
@prefix rdf: <http://www.w3.org/1999/02/22-rdf-syntax-ns#> .
@prefix owl: <http://www.w3.org/2002/07/owl#> .
@prefix xsd: <http://www.w3.org/2001/XMLSchema#> .
@prefix skos: <http://www.w3.org/2004/02/skos/core#> .
@prefix rdfs: <http://www.w3.org/2000/01/rdf-schema#> .

iss-spae:SafetyPerformanceAssessmentElements
    cc:license <https://creativecommons.org/licenses/by/4.0/> ;
    dct:issued "2025-04-07"^^xsd:date ;
    dct:title "Concept scheme grouping safety performance assessement elements "@en ;
    rdf:type skos:ConceptScheme ;
    rdfs:comment "Controlled SKOS-based vocabulary defined by the European Union Agency for Railways to describe concepts related to the Information Sharing System (ISS) in accordance with the draft delegated act of the future CSM ASLP Regulation."@en ;
    rdfs:label "Safety Performance Assessement Elements "@en ;
    skos:prefLabel "Safety Performance Assessement Elements "@en .

<http://data.europa.eu/949/concepts/safety-performance-assessment-elements/1>
    rdf:type skos:Concept ;
    skos:definition "PLAN"@en ;
    skos:inScheme iss-spae:SafetyPerformanceAssessmentElements ;
    skos:notation "P" ;
    skos:prefLabel "PLAN"@en .

<http://data.europa.eu/949/concepts/safety-performance-assessment-elements/1.2>
    rdf:type skos:Concept ;
    skos:broader <http://data.europa.eu/949/concepts/safety-performance-assessment-elements/1> ;
    skos:definition "PLAN-L2"@en ;
    skos:inScheme iss-spae:SafetyPerformanceAssessmentElements ;
    skos:notation "P-L2" ;
    skos:prefLabel "Level 2"@en .

<http://data.europa.eu/949/concepts/safety-performance-assessment-elements/1.2.1>
    rdf:type skos:Concept ;
    skos:broader <http://data.europa.eu/949/concepts/safety-performance-assessment-elements/1.2> ;
    skos:definition "The hazard record includes all hazards, together with all related RCM and system assumptions identified during the risk assessment process. It contains a clear reference to the origin of the hazards and to the selected risk acceptance principles."@en ;
    skos:inScheme iss-spae:SafetyPerformanceAssessmentElements ;
    skos:notation "P-L2-E.1" ;
    skos:prefLabel "P-L2-E.1-The hazard record includes all hazards, together with all related RCM and system assumptions identified during the risk assessment process. It contains a clear reference to the origin of the hazards and to the selected risk acceptance principles."@en .

<http://data.europa.eu/949/concepts/safety-performance-assessment-elements/1.2.2>
    rdf:type skos:Concept ;
    skos:broader <http://data.europa.eu/949/concepts/safety-performance-assessment-elements/1.2> ;
    skos:definition "Process for risk assessment documented."@en ;
    skos:inScheme iss-spae:SafetyPerformanceAssessmentElements ;
    skos:notation "P-L2-E.2" ;
    skos:prefLabel "P-L2-E.2-Process for risk assessment documented."@en .

<http://data.europa.eu/949/concepts/safety-performance-assessment-elements/1.2.3>
    rdf:type skos:Concept ;
    skos:broader <http://data.europa.eu/949/concepts/safety-performance-assessment-elements/1.2> ;
    skos:definition "Overview of training of staff members with regard to risk assessment."@en ;
    skos:inScheme iss-spae:SafetyPerformanceAssessmentElements ;
    skos:notation "P-L2-E.3" ;
    skos:prefLabel "P-L2-E.3-Overview of training of staff members with regard to risk assessment."@en .

<http://data.europa.eu/949/concepts/safety-performance-assessment-elements/1.2.4>
    rdf:type skos:Concept ;
    skos:broader <http://data.europa.eu/949/concepts/safety-performance-assessment-elements/1.2> ;
    skos:definition "Process for change management documented."@en ;
    skos:inScheme iss-spae:SafetyPerformanceAssessmentElements ;
    skos:notation "P-L2-E.4" ;
    skos:prefLabel "P-L2-E.4-Process for change management documented."@en .

<http://data.europa.eu/949/concepts/safety-performance-assessment-elements/1.2.5>
    rdf:type skos:Concept ;
    skos:broader <http://data.europa.eu/949/concepts/safety-performance-assessment-elements/1.2> ;
    skos:definition "Overview of assessed risk scenarios (serious risks for safety)."@en ;
    skos:inScheme iss-spae:SafetyPerformanceAssessmentElements ;
    skos:notation "P-L2-E.5" ;
    skos:prefLabel "P-L2-E.5-Overview of assessed risk scenarios (serious risks for safety)."@en .

<http://data.europa.eu/949/concepts/safety-performance-assessment-elements/1.2.6>
    rdf:type skos:Concept ;
    skos:broader <http://data.europa.eu/949/concepts/safety-performance-assessment-elements/1.2> ;
    skos:definition "Risk assessment of operational processes is performed by staff together knowledgeable of risk assessment as well as the assessed operational process."@en ;
    skos:inScheme iss-spae:SafetyPerformanceAssessmentElements ;
    skos:notation "P-L2-E.6" ;
    skos:prefLabel "P-L2-E.6-Risk assessment of operational processes is performed by staff together knowledgeable of risk assessment as well as the assessed operational process."@en .

<http://data.europa.eu/949/concepts/safety-performance-assessment-elements/1.2.7>
    rdf:type skos:Concept ;
    skos:broader <http://data.europa.eu/949/concepts/safety-performance-assessment-elements/1.2> ;
    skos:definition "The company deploys staff with knowledge of Human and Organisational Factors concepts that can be mobilized in risk management processes."@en ;
    skos:inScheme iss-spae:SafetyPerformanceAssessmentElements ;
    skos:notation "P-L2-E.7" ;
    skos:prefLabel "P-L2-E.7-The company deploys staff with knowledge of Human and Organisational Factors concepts that can be mobilized in risk management processes."@en .

<http://data.europa.eu/949/concepts/safety-performance-assessment-elements/1.2.8>
    rdf:type skos:Concept ;
    skos:broader <http://data.europa.eu/949/concepts/safety-performance-assessment-elements/1.2> ;
    skos:definition "Evidence that the change management process systematically involves a risk management process."@en ;
    skos:inScheme iss-spae:SafetyPerformanceAssessmentElements ;
    skos:notation "P-L2-E.8" ;
    skos:prefLabel "P-L2-E.8-Evidence that the change management process systematically involves a risk management process."@en .

<http://data.europa.eu/949/concepts/safety-performance-assessment-elements/1.2.9>
    rdf:type skos:Concept ;
    skos:broader <http://data.europa.eu/949/concepts/safety-performance-assessment-elements/1.2> ;
    skos:definition "The 10 most important risk control measures described in accordance with the part 1 and the part 2 of the applicable dataset in section 2.2 of Appendix B – Part B and limited to the prevented events."@en ;
    skos:inScheme iss-spae:SafetyPerformanceAssessmentElements ;
    skos:notation "P-L2-E.9" ;
    skos:prefLabel "P-L2-E.9-The 10 most important risk control measures described in accordance with the part 1 and the part 2 of the applicable dataset in section 2.2 of Appendix B – Part B and limited to the prevented events."@en .

<http://data.europa.eu/949/concepts/safety-performance-assessment-elements/1.3>
    rdf:type skos:Concept ;
    skos:broader <http://data.europa.eu/949/concepts/safety-performance-assessment-elements/1> ;
    skos:definition "PLAN-L3"@en ;
    skos:inScheme iss-spae:SafetyPerformanceAssessmentElements ;
    skos:notation "P-L3" ;
    skos:prefLabel "Level 3"@en .

<http://data.europa.eu/949/concepts/safety-performance-assessment-elements/1.3.1>
    rdf:type skos:Concept ;
    skos:broader <http://data.europa.eu/949/concepts/safety-performance-assessment-elements/1.3> ;
    skos:definition "Operator uses acceptance criteria in risk-based decision-making."@en ;
    skos:inScheme iss-spae:SafetyPerformanceAssessmentElements ;
    skos:notation "P-L3-E.10" ;
    skos:prefLabel "P-L3-E.10-Operator uses acceptance criteria in risk-based decision-making."@en .

<http://data.europa.eu/949/concepts/safety-performance-assessment-elements/1.3.2>
    rdf:type skos:Concept ;
    skos:broader <http://data.europa.eu/949/concepts/safety-performance-assessment-elements/1.3> ;
    skos:definition "Process for the identification of risks associated with human and organisational factors during the risk assessment process."@en ;
    skos:inScheme iss-spae:SafetyPerformanceAssessmentElements ;
    skos:notation "P-L3-E.11" ;
    skos:prefLabel "P-L3-E.11-Process for the identification of risks associated with human and organisational factors during the risk assessment process."@en .

<http://data.europa.eu/949/concepts/safety-performance-assessment-elements/1.3.3>
    rdf:type skos:Concept ;
    skos:broader <http://data.europa.eu/949/concepts/safety-performance-assessment-elements/1.3> ;
    skos:definition "Elements exist that human and organisational factors are taken into consideration in the risk assessment process and the change management process (evidence of application of process – see 11.)."@en ;
    skos:inScheme iss-spae:SafetyPerformanceAssessmentElements ;
    skos:notation "P-L3-E.12" ;
    skos:prefLabel "P-L3-E.12-Elements exist that human and organisational factors are taken into consideration in the risk assessment process and the change management process (evidence of application of process – see 11.)."@en .

<http://data.europa.eu/949/concepts/safety-performance-assessment-elements/1.3.4>
    rdf:type skos:Concept ;
    skos:broader <http://data.europa.eu/949/concepts/safety-performance-assessment-elements/1.3> ;
    skos:definition "Overview of assessed risk scenario’s concerning all the risks for safety that are identified the railway operator."@en ;
    skos:inScheme iss-spae:SafetyPerformanceAssessmentElements ;
    skos:notation "P-L3-E.13" ;
    skos:prefLabel "P-L3-E.13-Overview of assessed risk scenario’s concerning all the risks for safety that are identified the railway operator."@en .

<http://data.europa.eu/949/concepts/safety-performance-assessment-elements/1.3.5>
    rdf:type skos:Concept ;
    skos:broader <http://data.europa.eu/949/concepts/safety-performance-assessment-elements/1.3> ;
    skos:definition "The 10 most important risk control measures described in accordance with the parts 1, 2 and 3 of the applicable dataset in section 2.2 of Appendix B – Part B."@en ;
    skos:inScheme iss-spae:SafetyPerformanceAssessmentElements ;
    skos:notation "P-L3-E.14" ;
    skos:prefLabel "P-L3-E.14-The 10 most important risk control measures described in accordance with the parts 1, 2 and 3 of the applicable dataset in section 2.2 of Appendix B – Part B."@en .

<http://data.europa.eu/949/concepts/safety-performance-assessment-elements/1.4>
    rdf:type skos:Concept ;
    skos:broader <http://data.europa.eu/949/concepts/safety-performance-assessment-elements/1> ;
    skos:definition "PLAN-L4"@en ;
    skos:inScheme iss-spae:SafetyPerformanceAssessmentElements ;
    skos:notation "P-L4" ;
    skos:prefLabel "Level 4"@en .

<http://data.europa.eu/949/concepts/safety-performance-assessment-elements/1.4.1>
    rdf:type skos:Concept ;
    skos:broader <http://data.europa.eu/949/concepts/safety-performance-assessment-elements/1.4> ;
    skos:definition "Performance indicators are measured regarding the risk assessment process."@en ;
    skos:inScheme iss-spae:SafetyPerformanceAssessmentElements ;
    skos:notation "P-L4-E.15" ;
    skos:prefLabel "P-L4-E.15-Performance indicators are measured regarding the risk assessment process."@en .

<http://data.europa.eu/949/concepts/safety-performance-assessment-elements/1.4.2>
    rdf:type skos:Concept ;
    skos:broader <http://data.europa.eu/949/concepts/safety-performance-assessment-elements/1.4> ;
    skos:definition "Periodic review meetings regarding the risk assessment process take place."@en ;
    skos:inScheme iss-spae:SafetyPerformanceAssessmentElements ;
    skos:notation "P-L4-E.16" ;
    skos:prefLabel "P-L4-E.16-Periodic review meetings regarding the risk assessment process take place."@en .

<http://data.europa.eu/949/concepts/safety-performance-assessment-elements/1.4.3>
    rdf:type skos:Concept ;
    skos:broader <http://data.europa.eu/949/concepts/safety-performance-assessment-elements/1.4> ;
    skos:definition "Reviews are undertaken of the expertise present during risk analyses with respect to the topics under analysis."@en ;
    skos:inScheme iss-spae:SafetyPerformanceAssessmentElements ;
    skos:notation "P-L4-E.17" ;
    skos:prefLabel "P-L4-E.17-Reviews are undertaken of the expertise present during risk analyses with respect to the topics under analysis."@en .

<http://data.europa.eu/949/concepts/safety-performance-assessment-elements/1.4.4>
    rdf:type skos:Concept ;
    skos:broader <http://data.europa.eu/949/concepts/safety-performance-assessment-elements/1.4> ;
    skos:definition "The 10 most important risk control measures described in accordance with the parts 1, 2, 3 and 4 of the applicable dataset in section 2.2 of Appendix B – Part B."@en ;
    skos:inScheme iss-spae:SafetyPerformanceAssessmentElements ;
    skos:notation "P-L4-E.18" ;
    skos:prefLabel "P-L4-E.18-The 10 most important risk control measures described in accordance with the parts 1, 2, 3 and 4 of the applicable dataset in section 2.2 of Appendix B – Part B."@en .

<http://data.europa.eu/949/concepts/safety-performance-assessment-elements/1.5>
    rdf:type skos:Concept ;
    skos:broader <http://data.europa.eu/949/concepts/safety-performance-assessment-elements/1> ;
    skos:definition "PLAN-L5"@en ;
    skos:inScheme iss-spae:SafetyPerformanceAssessmentElements ;
    skos:notation "P-L5" ;
    skos:prefLabel "Level 5"@en .

<http://data.europa.eu/949/concepts/safety-performance-assessment-elements/1.5.1>
    rdf:type skos:Concept ;
    skos:broader <http://data.europa.eu/949/concepts/safety-performance-assessment-elements/1.5> ;
    skos:definition "The railway operator regularly conducts in-depth reviews of its risk assessment methods and adapts them in function of these findings."@en ;
    skos:inScheme iss-spae:SafetyPerformanceAssessmentElements ;
    skos:notation "P-L5-E.19" ;
    skos:prefLabel "P-L5-E.19-The railway operator regularly conducts in-depth reviews of its risk assessment methods and adapts them in function of these findings."@en .

<http://data.europa.eu/949/concepts/safety-performance-assessment-elements/1.5.2>
    rdf:type skos:Concept ;
    skos:broader <http://data.europa.eu/949/concepts/safety-performance-assessment-elements/1.5> ;
    skos:definition "Human and organisational factors issues are fully integrated in the risk assessment process and the change management process and are continuously reviewed."@en ;
    skos:inScheme iss-spae:SafetyPerformanceAssessmentElements ;
    skos:notation "P-L5-E.20" ;
    skos:prefLabel "P-L5-E.20-Human and organisational factors issues are fully integrated in the risk assessment process and the change management process and are continuously reviewed."@en .

<http://data.europa.eu/949/concepts/safety-performance-assessment-elements/1.5.3>
    rdf:type skos:Concept ;
    skos:broader <http://data.europa.eu/949/concepts/safety-performance-assessment-elements/1.5> ;
    skos:definition "The 20 most important risk control measures described in accordance with the parts 1, 2, 3 and 4 of the applicable dataset in section 2.2 of Appendix B – Part B. "@en ;
    skos:inScheme iss-spae:SafetyPerformanceAssessmentElements ;
    skos:notation "P-L5-E.21" ;
    skos:prefLabel "P-L5-E.21-The 20 most important risk control measures described in accordance with the parts 1, 2, 3 and 4 of the applicable dataset in section 2.2 of Appendix B – Part B. "@en .

<http://data.europa.eu/949/concepts/safety-performance-assessment-elements/2>
    rdf:type skos:Concept ;
    skos:definition "DO"@en ;
    skos:inScheme iss-spae:SafetyPerformanceAssessmentElements ;
    skos:notation "D" ;
    skos:prefLabel "DO"@en .

<http://data.europa.eu/949/concepts/safety-performance-assessment-elements/2.2>
    rdf:type skos:Concept ;
    skos:broader <http://data.europa.eu/949/concepts/safety-performance-assessment-elements/2> ;
    skos:definition "DO-L2"@en ;
    skos:inScheme iss-spae:SafetyPerformanceAssessmentElements ;
    skos:notation "D-L2" ;
    skos:prefLabel "Level 2"@en .

<http://data.europa.eu/949/concepts/safety-performance-assessment-elements/2.2.1>
    rdf:type skos:Concept ;
    skos:broader <http://data.europa.eu/949/concepts/safety-performance-assessment-elements/2.2> ;
    skos:definition "The railway operator informs its staff (and external staff concerned) of the risks and RCM relevant for their activities."@en ;
    skos:inScheme iss-spae:SafetyPerformanceAssessmentElements ;
    skos:notation "D-L2-E.22" ;
    skos:prefLabel "D-L2-E.22-The railway operator informs its staff (and external staff concerned) of the risks and RCM relevant for their activities."@en .

<http://data.europa.eu/949/concepts/safety-performance-assessment-elements/2.2.2>
    rdf:type skos:Concept ;
    skos:broader <http://data.europa.eu/949/concepts/safety-performance-assessment-elements/2.2> ;
    skos:definition "The demonstration is made that the risk control measures in place have an assigned responsible(s) in charge of operating and maintaining them."@en ;
    skos:inScheme iss-spae:SafetyPerformanceAssessmentElements ;
    skos:notation "D-L2-E.23" ;
    skos:prefLabel "D-L2-E.23-The demonstration is made that the risk control measures in place have an assigned responsible(s) in charge of operating and maintaining them."@en .

<http://data.europa.eu/949/concepts/safety-performance-assessment-elements/2.2.3>
    rdf:type skos:Concept ;
    skos:broader <http://data.europa.eu/949/concepts/safety-performance-assessment-elements/2.2> ;
    skos:definition "The competence management system ensures staff has the competences needed to implement, operate and maintain risk control measures."@en ;
    skos:inScheme iss-spae:SafetyPerformanceAssessmentElements ;
    skos:notation "D-L2-E.24" ;
    skos:prefLabel "D-L2-E.24-The competence management system ensures staff has the competences needed to implement, operate and maintain risk control measures."@en .

<http://data.europa.eu/949/concepts/safety-performance-assessment-elements/2.2.4>
    rdf:type skos:Concept ;
    skos:broader <http://data.europa.eu/949/concepts/safety-performance-assessment-elements/2.2> ;
    skos:definition "The operation of risk control measures and expected performance refers clearly to the system assumptions identified during the risk assessment process and contains a clear reference to the origin of the hazards."@en ;
    skos:inScheme iss-spae:SafetyPerformanceAssessmentElements ;
    skos:notation "D-L2-E.25" ;
    skos:prefLabel "D-L2-E.25-The operation of risk control measures and expected performance refers clearly to the system assumptions identified during the risk assessment process and contains a clear reference to the origin of the hazards."@en .

<http://data.europa.eu/949/concepts/safety-performance-assessment-elements/2.2.5>
    rdf:type skos:Concept ;
    skos:broader <http://data.europa.eu/949/concepts/safety-performance-assessment-elements/2.2> ;
    skos:definition "The demonstration is made that records of decisions taken by the railway operator take safety into consideration."@en ;
    skos:inScheme iss-spae:SafetyPerformanceAssessmentElements ;
    skos:notation "D-L2-E.26" ;
    skos:prefLabel "D-L2-E.26-The demonstration is made that records of decisions taken by the railway operator take safety into consideration."@en .

<http://data.europa.eu/949/concepts/safety-performance-assessment-elements/2.3>
    rdf:type skos:Concept ;
    skos:broader <http://data.europa.eu/949/concepts/safety-performance-assessment-elements/2> ;
    skos:definition "DO-L3"@en ;
    skos:inScheme iss-spae:SafetyPerformanceAssessmentElements ;
    skos:notation "D-L3" ;
    skos:prefLabel "Level 3"@en .

<http://data.europa.eu/949/concepts/safety-performance-assessment-elements/2.3.1>
    rdf:type skos:Concept ;
    skos:broader <http://data.europa.eu/949/concepts/safety-performance-assessment-elements/2.3> ;
    skos:definition "Arrangements exist on managing shared risks and responsibilities."@en ;
    skos:inScheme iss-spae:SafetyPerformanceAssessmentElements ;
    skos:notation "D-L3-E.27" ;
    skos:prefLabel "D-L3-E.27-Arrangements exist on managing shared risks and responsibilities."@en .

<http://data.europa.eu/949/concepts/safety-performance-assessment-elements/2.3.2>
    rdf:type skos:Concept ;
    skos:broader <http://data.europa.eu/949/concepts/safety-performance-assessment-elements/2.3> ;
    skos:definition "A distinction is made between the type of risk control measure: RCMs that prevent occurrences, RCMs that reduce the severity of consequences."@en ;
    skos:inScheme iss-spae:SafetyPerformanceAssessmentElements ;
    skos:notation "D-L3-E.28" ;
    skos:prefLabel "D-L3-E.28-A distinction is made between the type of risk control measure: RCMs that prevent occurrences, RCMs that reduce the severity of consequences."@en .

<http://data.europa.eu/949/concepts/safety-performance-assessment-elements/2.3.3>
    rdf:type skos:Concept ;
    skos:broader <http://data.europa.eu/949/concepts/safety-performance-assessment-elements/2.3> ;
    skos:definition "A method exists that considers both the effort as well as the benefits of the risk control measures to be able to prioritize measures based on resource-effectiveness. (Goal: Resources for risk reduction are allocated to maximize the resulting risk reduction)."@en ;
    skos:inScheme iss-spae:SafetyPerformanceAssessmentElements ;
    skos:notation "D-L3-E.29" ;
    skos:prefLabel "D-L3-E.29-A method exists that considers both the effort as well as the benefits of the risk control measures to be able to prioritize measures based on resource-effectiveness. (Goal: Resources for risk reduction are allocated to maximize the resulting risk reduction)."@en .

<http://data.europa.eu/949/concepts/safety-performance-assessment-elements/2.4>
    rdf:type skos:Concept ;
    skos:broader <http://data.europa.eu/949/concepts/safety-performance-assessment-elements/2> ;
    skos:definition "DO-L4"@en ;
    skos:inScheme iss-spae:SafetyPerformanceAssessmentElements ;
    skos:notation "D-L4" ;
    skos:prefLabel "Level 4"@en .

<http://data.europa.eu/949/concepts/safety-performance-assessment-elements/2.4.1>
    rdf:type skos:Concept ;
    skos:broader <http://data.europa.eu/949/concepts/safety-performance-assessment-elements/2.4> ;
    skos:definition "There is evidence to estimate the effects of risk control measures across multiple risks (e.g. risks identified in multiple risk assessments)."@en ;
    skos:inScheme iss-spae:SafetyPerformanceAssessmentElements ;
    skos:notation "D-L4-E.30" ;
    skos:prefLabel "D-L4-E.30-There is evidence to estimate the effects of risk control measures across multiple risks (e.g. risks identified in multiple risk assessments)."@en .

<http://data.europa.eu/949/concepts/safety-performance-assessment-elements/2.4.2>
    rdf:type skos:Concept ;
    skos:broader <http://data.europa.eu/949/concepts/safety-performance-assessment-elements/2.4> ;
    skos:definition "The method for assessing the resource effectiveness of RCM is systematically applied."@en ;
    skos:inScheme iss-spae:SafetyPerformanceAssessmentElements ;
    skos:notation "D-L4-E.31" ;
    skos:prefLabel "D-L4-E.31-The method for assessing the resource effectiveness of RCM is systematically applied."@en .

<http://data.europa.eu/949/concepts/safety-performance-assessment-elements/2.4.3>
    rdf:type skos:Concept ;
    skos:broader <http://data.europa.eu/949/concepts/safety-performance-assessment-elements/2.4> ;
    skos:definition "Management systems for different topics (such as safety) are integrated."@en ;
    skos:inScheme iss-spae:SafetyPerformanceAssessmentElements ;
    skos:notation "D-L4-E.32" ;
    skos:prefLabel "D-L4-E.32-Management systems for different topics (such as safety) are integrated."@en .

<http://data.europa.eu/949/concepts/safety-performance-assessment-elements/2.5>
    rdf:type skos:Concept ;
    skos:broader <http://data.europa.eu/949/concepts/safety-performance-assessment-elements/2> ;
    skos:definition "DO-L5"@en ;
    skos:inScheme iss-spae:SafetyPerformanceAssessmentElements ;
    skos:notation "D-L5" ;
    skos:prefLabel "Level 5"@en .

<http://data.europa.eu/949/concepts/safety-performance-assessment-elements/2.5.1>
    rdf:type skos:Concept ;
    skos:broader <http://data.europa.eu/949/concepts/safety-performance-assessment-elements/2.5> ;
    skos:definition "Description of the decision making process at strategic level that includes a risk-based approach. "@en ;
    skos:inScheme iss-spae:SafetyPerformanceAssessmentElements ;
    skos:notation "D-L5-E.33" ;
    skos:prefLabel "D-L5-E.33-Description of the decision making process at strategic level that includes a risk-based approach. "@en .

<http://data.europa.eu/949/concepts/safety-performance-assessment-elements/3>
    rdf:type skos:Concept ;
    skos:definition "CHECK"@en ;
    skos:inScheme iss-spae:SafetyPerformanceAssessmentElements ;
    skos:notation "C" ;
    skos:prefLabel "CHECK"@en .

<http://data.europa.eu/949/concepts/safety-performance-assessment-elements/3.2>
    rdf:type skos:Concept ;
    skos:broader <http://data.europa.eu/949/concepts/safety-performance-assessment-elements/3> ;
    skos:definition "CHECK-L2"@en ;
    skos:inScheme iss-spae:SafetyPerformanceAssessmentElements ;
    skos:notation "C-L2" ;
    skos:prefLabel "Level 2"@en .

<http://data.europa.eu/949/concepts/safety-performance-assessment-elements/3.2.1>
    rdf:type skos:Concept ;
    skos:broader <http://data.europa.eu/949/concepts/safety-performance-assessment-elements/3.2> ;
    skos:definition "The monitoring plan considers the risk control measures in areas that give rise to serious risks and if these measures are not monitored effectively, this could lead to adverse consequences for safety."@en ;
    skos:inScheme iss-spae:SafetyPerformanceAssessmentElements ;
    skos:notation "C-L2-E.34" ;
    skos:prefLabel "C-L2-E.34-The monitoring plan considers the risk control measures in areas that give rise to serious risks and if these measures are not monitored effectively, this could lead to adverse consequences for safety."@en .

<http://data.europa.eu/949/concepts/safety-performance-assessment-elements/3.3>
    rdf:type skos:Concept ;
    skos:broader <http://data.europa.eu/949/concepts/safety-performance-assessment-elements/3> ;
    skos:definition "CHECK-L3"@en ;
    skos:inScheme iss-spae:SafetyPerformanceAssessmentElements ;
    skos:notation "C-L3" ;
    skos:prefLabel "Level 3"@en .

<http://data.europa.eu/949/concepts/safety-performance-assessment-elements/3.3.1>
    rdf:type skos:Concept ;
    skos:broader <http://data.europa.eu/949/concepts/safety-performance-assessment-elements/3.3> ;
    skos:definition "The monitoring plan considers all monitorable and necessary risk control measures. The monitoring plan yields robust and reproducible results."@en ;
    skos:inScheme iss-spae:SafetyPerformanceAssessmentElements ;
    skos:notation "C-L3-E.35" ;
    skos:prefLabel "C-L3-E.35-The monitoring plan considers all monitorable and necessary risk control measures. The monitoring plan yields robust and reproducible results."@en .

<http://data.europa.eu/949/concepts/safety-performance-assessment-elements/3.3.2>
    rdf:type skos:Concept ;
    skos:broader <http://data.europa.eu/949/concepts/safety-performance-assessment-elements/3.3> ;
    skos:definition "The performance of each RCMs is monitored using pre-defined indicators that give information regarding its effectiveness. "@en ;
    skos:inScheme iss-spae:SafetyPerformanceAssessmentElements ;
    skos:notation "C-L3-E.36" ;
    skos:prefLabel "C-L3-E.36-The performance of each RCMs is monitored using pre-defined indicators that give information regarding its effectiveness. "@en .

<http://data.europa.eu/949/concepts/safety-performance-assessment-elements/3.3.3>
    rdf:type skos:Concept ;
    skos:broader <http://data.europa.eu/949/concepts/safety-performance-assessment-elements/3.3> ;
    skos:definition "The railway operator systematically monitors the risk control measures and identifies their weaknesses."@en ;
    skos:inScheme iss-spae:SafetyPerformanceAssessmentElements ;
    skos:notation "C-L3-E.37" ;
    skos:prefLabel "C-L3-E.37-The railway operator systematically monitors the risk control measures and identifies their weaknesses."@en .

<http://data.europa.eu/949/concepts/safety-performance-assessment-elements/3.4>
    rdf:type skos:Concept ;
    skos:broader <http://data.europa.eu/949/concepts/safety-performance-assessment-elements/3> ;
    skos:definition "CHECK-L4"@en ;
    skos:inScheme iss-spae:SafetyPerformanceAssessmentElements ;
    skos:notation "C-L4" ;
    skos:prefLabel "Level 4"@en .

<http://data.europa.eu/949/concepts/safety-performance-assessment-elements/3.4.1>
    rdf:type skos:Concept ;
    skos:broader <http://data.europa.eu/949/concepts/safety-performance-assessment-elements/3.4> ;
    skos:definition "The management supports a culture in which both positive and negative experiences on the perception of risk levels are openly shared and discussed for learning."@en ;
    skos:inScheme iss-spae:SafetyPerformanceAssessmentElements ;
    skos:notation "C-L4-E.38" ;
    skos:prefLabel "C-L4-E.38-The management supports a culture in which both positive and negative experiences on the perception of risk levels are openly shared and discussed for learning."@en .

<http://data.europa.eu/949/concepts/safety-performance-assessment-elements/3.4.2>
    rdf:type skos:Concept ;
    skos:broader <http://data.europa.eu/949/concepts/safety-performance-assessment-elements/3.4> ;
    skos:definition "The majority of important risks are monitored using leading indicators."@en ;
    skos:inScheme iss-spae:SafetyPerformanceAssessmentElements ;
    skos:notation "C-L4-E.39" ;
    skos:prefLabel "C-L4-E.39-The majority of important risks are monitored using leading indicators."@en .

<http://data.europa.eu/949/concepts/safety-performance-assessment-elements/3.4.3>
    rdf:type skos:Concept ;
    skos:broader <http://data.europa.eu/949/concepts/safety-performance-assessment-elements/3.4> ;
    skos:definition "Reporting is available on the coherent and correct application of the risk assessment process and the change management process."@en ;
    skos:inScheme iss-spae:SafetyPerformanceAssessmentElements ;
    skos:notation "C-L4-E.40" ;
    skos:prefLabel "C-L4-E.40-Reporting is available on the coherent and correct application of the risk assessment process and the change management process."@en .

<http://data.europa.eu/949/concepts/safety-performance-assessment-elements/3.4.4>
    rdf:type skos:Concept ;
    skos:broader <http://data.europa.eu/949/concepts/safety-performance-assessment-elements/3.4> ;
    skos:definition "Best practices stemming from other industries are sought after and incorporated, if relevant. "@en ;
    skos:inScheme iss-spae:SafetyPerformanceAssessmentElements ;
    skos:notation "C-L4-E.41" ;
    skos:prefLabel "C-L4-E.41-Best practices stemming from other industries are sought after and incorporated, if relevant. "@en .

<http://data.europa.eu/949/concepts/safety-performance-assessment-elements/3.5>
    rdf:type skos:Concept ;
    skos:broader <http://data.europa.eu/949/concepts/safety-performance-assessment-elements/3> ;
    skos:definition "CHECK-L5"@en ;
    skos:inScheme iss-spae:SafetyPerformanceAssessmentElements ;
    skos:notation "C-L5" ;
    skos:prefLabel "Level 5"@en .

<http://data.europa.eu/949/concepts/safety-performance-assessment-elements/3.5.1>
    rdf:type skos:Concept ;
    skos:broader <http://data.europa.eu/949/concepts/safety-performance-assessment-elements/3.5> ;
    skos:definition "Where possible, the railway operator has put in place a system for real-time automated data collection and monitoring with regard to monitoring of RCM’s."@en ;
    skos:inScheme iss-spae:SafetyPerformanceAssessmentElements ;
    skos:notation "C-L5-E.42" ;
    skos:prefLabel "C-L5-E.42-Where possible, the railway operator has put in place a system for real-time automated data collection and monitoring with regard to monitoring of RCM’s."@en .

<http://data.europa.eu/949/concepts/safety-performance-assessment-elements/3.5.2>
    rdf:type skos:Concept ;
    skos:broader <http://data.europa.eu/949/concepts/safety-performance-assessment-elements/3.5> ;
    skos:definition "The system ensures that the data is available when needed."@en ;
    skos:inScheme iss-spae:SafetyPerformanceAssessmentElements ;
    skos:notation "C-L5-E.43" ;
    skos:prefLabel "C-L5-E.43-The system ensures that the data is available when needed."@en .

<http://data.europa.eu/949/concepts/safety-performance-assessment-elements/3.5.3>
    rdf:type skos:Concept ;
    skos:broader <http://data.europa.eu/949/concepts/safety-performance-assessment-elements/3.5> ;
    skos:definition "The railway operator proactively organizes the sharing of lessons learned on the efficiency or effectiveness of risk control measures with external stakeholders (such as peers)."@en ;
    skos:inScheme iss-spae:SafetyPerformanceAssessmentElements ;
    skos:notation "C-L5-E.44" ;
    skos:prefLabel "C-L5-E.44-The railway operator proactively organizes the sharing of lessons learned on the efficiency or effectiveness of risk control measures with external stakeholders (such as peers)."@en .

<http://data.europa.eu/949/concepts/safety-performance-assessment-elements/3.5.4>
    rdf:type skos:Concept ;
    skos:broader <http://data.europa.eu/949/concepts/safety-performance-assessment-elements/3.5> ;
    skos:definition "Reporting is available on the coherent and systematic application of risk based decision making criteria and decision making process."@en ;
    skos:inScheme iss-spae:SafetyPerformanceAssessmentElements ;
    skos:notation "C-L5-E.45" ;
    skos:prefLabel "C-L5-E.45-Reporting is available on the coherent and systematic application of risk based decision making criteria and decision making process."@en .

<http://data.europa.eu/949/concepts/safety-performance-assessment-elements/4>
    rdf:type skos:Concept ;
    skos:definition "ACT"@en ;
    skos:inScheme iss-spae:SafetyPerformanceAssessmentElements ;
    skos:notation "A" ;
    skos:prefLabel "ACT"@en .

<http://data.europa.eu/949/concepts/safety-performance-assessment-elements/4.2>
    rdf:type skos:Concept ;
    skos:broader <http://data.europa.eu/949/concepts/safety-performance-assessment-elements/4> ;
    skos:definition "ACT-L2"@en ;
    skos:inScheme iss-spae:SafetyPerformanceAssessmentElements ;
    skos:notation "A-L2" ;
    skos:prefLabel "Level 2"@en .

<http://data.europa.eu/949/concepts/safety-performance-assessment-elements/4.2.1>
    rdf:type skos:Concept ;
    skos:broader <http://data.europa.eu/949/concepts/safety-performance-assessment-elements/4.2> ;
    skos:definition "Reports of ad-hoc reviews of risk assessments following the results of the monitoring activities."@en ;
    skos:inScheme iss-spae:SafetyPerformanceAssessmentElements ;
    skos:notation "A-L2-E.46" ;
    skos:prefLabel "A-L2-E.46-Reports of ad-hoc reviews of risk assessments following the results of the monitoring activities."@en .

<http://data.europa.eu/949/concepts/safety-performance-assessment-elements/4.2.2>
    rdf:type skos:Concept ;
    skos:broader <http://data.europa.eu/949/concepts/safety-performance-assessment-elements/4.2> ;
    skos:definition "Reports showing that relevant incidents and accidents are taken into account in the review (of risk assessment)."@en ;
    skos:inScheme iss-spae:SafetyPerformanceAssessmentElements ;
    skos:notation "A-L2-E.47" ;
    skos:prefLabel "A-L2-E.47-Reports showing that relevant incidents and accidents are taken into account in the review (of risk assessment)."@en .

<http://data.europa.eu/949/concepts/safety-performance-assessment-elements/4.2.3>
    rdf:type skos:Concept ;
    skos:broader <http://data.europa.eu/949/concepts/safety-performance-assessment-elements/4.2> ;
    skos:definition "The interface between the process(es) for risk assessment and the process(es) decision-making is documented. "@en ;
    skos:inScheme iss-spae:SafetyPerformanceAssessmentElements ;
    skos:notation "A-L2-E.48" ;
    skos:prefLabel "A-L2-E.48-The interface between the process(es) for risk assessment and the process(es) decision-making is documented. "@en .

<http://data.europa.eu/949/concepts/safety-performance-assessment-elements/4.3>
    rdf:type skos:Concept ;
    skos:broader <http://data.europa.eu/949/concepts/safety-performance-assessment-elements/4> ;
    skos:definition "ACT-L3"@en ;
    skos:inScheme iss-spae:SafetyPerformanceAssessmentElements ;
    skos:notation "A-L3" ;
    skos:prefLabel "Level 3"@en .

<http://data.europa.eu/949/concepts/safety-performance-assessment-elements/4.3.1>
    rdf:type skos:Concept ;
    skos:broader <http://data.europa.eu/949/concepts/safety-performance-assessment-elements/4.3> ;
    skos:definition "Planning of review of risk assessments."@en ;
    skos:inScheme iss-spae:SafetyPerformanceAssessmentElements ;
    skos:notation "A-L3-E.49" ;
    skos:prefLabel "A-L3-E.49-Planning of review of risk assessments."@en .

<http://data.europa.eu/949/concepts/safety-performance-assessment-elements/4.3.2>
    rdf:type skos:Concept ;
    skos:broader <http://data.europa.eu/949/concepts/safety-performance-assessment-elements/4.3> ;
    skos:definition "Records of top level management decisions clearly show the risks involved and the decision whether to accept/mitigate them."@en ;
    skos:inScheme iss-spae:SafetyPerformanceAssessmentElements ;
    skos:notation "A-L3-E.50" ;
    skos:prefLabel "A-L3-E.50-Records of top level management decisions clearly show the risks involved and the decision whether to accept/mitigate them."@en .

<http://data.europa.eu/949/concepts/safety-performance-assessment-elements/4.3.3>
    rdf:type skos:Concept ;
    skos:broader <http://data.europa.eu/949/concepts/safety-performance-assessment-elements/4.3> ;
    skos:definition "Learnings from monitoring process are used in the risk analyses. Risk analyses (risk calculations and/or risk identification) are updated in function of the learnings from monitoring. "@en ;
    skos:inScheme iss-spae:SafetyPerformanceAssessmentElements ;
    skos:notation "A-L3-E.51" ;
    skos:prefLabel "A-L3-E.51-Learnings from monitoring process are used in the risk analyses. Risk analyses (risk calculations and/or risk identification) are updated in function of the learnings from monitoring. "@en .

<http://data.europa.eu/949/concepts/safety-performance-assessment-elements/4.4>
    rdf:type skos:Concept ;
    skos:broader <http://data.europa.eu/949/concepts/safety-performance-assessment-elements/4> ;
    skos:definition "ACT-L4"@en ;
    skos:inScheme iss-spae:SafetyPerformanceAssessmentElements ;
    skos:notation "A-L4" ;
    skos:prefLabel "Level 4"@en .

<http://data.europa.eu/949/concepts/safety-performance-assessment-elements/4.4.1>
    rdf:type skos:Concept ;
    skos:broader <http://data.europa.eu/949/concepts/safety-performance-assessment-elements/4.4> ;
    skos:definition "Planning of reviews of risk assessments is risk-based and considers reported accident and incident occurrences rates."@en ;
    skos:inScheme iss-spae:SafetyPerformanceAssessmentElements ;
    skos:notation "A-L4-E.52" ;
    skos:prefLabel "A-L4-E.52-Planning of reviews of risk assessments is risk-based and considers reported accident and incident occurrences rates."@en .

<http://data.europa.eu/949/concepts/safety-performance-assessment-elements/4.4.2>
    rdf:type skos:Concept ;
    skos:broader <http://data.europa.eu/949/concepts/safety-performance-assessment-elements/4.4> ;
    skos:definition "The interface between the monitoring processes and the risk assessment processes guarantees a quick adjustment in the operational processes in case of predictive trends pointing towards a decline in safety performance. "@en ;
    skos:inScheme iss-spae:SafetyPerformanceAssessmentElements ;
    skos:notation "A-L4-E.53" ;
    skos:prefLabel "A-L4-E.53-The interface between the monitoring processes and the risk assessment processes guarantees a quick adjustment in the operational processes in case of predictive trends pointing towards a decline in safety performance. "@en .

<http://data.europa.eu/949/concepts/safety-performance-assessment-elements/4.5>
    rdf:type skos:Concept ;
    skos:broader <http://data.europa.eu/949/concepts/safety-performance-assessment-elements/4> ;
    skos:definition "ACT-L5"@en ;
    skos:inScheme iss-spae:SafetyPerformanceAssessmentElements ;
    skos:notation "A-L5" ;
    skos:prefLabel "Level 5"@en .

<http://data.europa.eu/949/concepts/safety-performance-assessment-elements/4.5.1>
    rdf:type skos:Concept ;
    skos:broader <http://data.europa.eu/949/concepts/safety-performance-assessment-elements/4.5> ;
    skos:definition "The organisation tracks continuously the evolution of its risk profile, which shows continuous improvement."@en ;
    skos:inScheme iss-spae:SafetyPerformanceAssessmentElements ;
    skos:notation "A-L5-E.54" ;
    skos:prefLabel "A-L5-E.54-The organisation tracks continuously the evolution of its risk profile, which shows continuous improvement."@en .

<http://data.europa.eu/949/concepts/safety-performance-assessment-elements/4.5.2>
    rdf:type skos:Concept ;
    skos:broader <http://data.europa.eu/949/concepts/safety-performance-assessment-elements/4.5> ;
    skos:definition "The top management takes a proactive role in developing, maintaining and improving the Safety Management System through regular review of internal measures, including staff communication as well as horizon scanning to identify new improvement opportunities."@en ;
    skos:inScheme iss-spae:SafetyPerformanceAssessmentElements ;
    skos:notation "A-L5-E.55" ;
    skos:prefLabel "A-L5-E.55-The top management takes a proactive role in developing, maintaining and improving the Safety Management System through regular review of internal measures, including staff communication as well as horizon scanning to identify new improvement opportunities."@en .

<http://data.europa.eu/949/concepts/safety-performance-assessment-elements/4.5.3>
    rdf:type skos:Concept ;
    skos:broader <http://data.europa.eu/949/concepts/safety-performance-assessment-elements/4.5> ;
    skos:definition "The way risks are managed is constantly challenged. The interface between the monitoring processes and the risk assessment processes ensures an improvement initiative in the applied risk management methods (continuous improvement of risk management activities). "@en ;
    skos:inScheme iss-spae:SafetyPerformanceAssessmentElements ;
    skos:notation "A-L5-E.56" ;
    skos:prefLabel "A-L5-E.56-The way risks are managed is constantly challenged. The interface between the monitoring processes and the risk assessment processes ensures an improvement initiative in the applied risk management methods (continuous improvement of risk management activities). "@en .

